rt ainvs: add conjunct to valid_refills
This conjunct says that every refill must have nonzero r_amount

Signed-off-by: Michael McInerney <m.mcinerney@unsw.edu.au>

proof/invariant-abstract/DetSchedSchedule_AI.thy
@@ -7041,9 +7041,10 @@ method merge_refills_simple
 
 lemma merge_refills_refills_sum:
   "\<lbrace>\<lambda>s. pred_map (\<lambda>cfg. refills_sum (scrc_refills cfg) = scrc_budget cfg)
-                 (sc_refill_cfgs_of s) sc_ptr
-        \<and> pred_map (\<lambda>cfg. 1 < length (scrc_refills cfg)) (sc_refill_cfgs_of s) sc_ptr\<rbrace>
-   merge_refills sc_ptr
+                                          (sc_refill_cfgs_of s) sc_ptr
+        \<and> (sc_ptr' = sc_ptr \<longrightarrow>  pred_map (\<lambda>cfg. 1 < length (scrc_refills cfg))
+                                          (sc_refill_cfgs_of s) sc_ptr)\<rbrace>
+   merge_refills sc_ptr'
    \<lbrace>\<lambda>_ s. pred_map (\<lambda>cfg. refills_sum (scrc_refills cfg) = scrc_budget cfg)
                  (sc_refill_cfgs_of s) sc_ptr\<rbrace>"
   apply merge_refills_simple
@@ -7052,22 +7053,33 @@ lemma merge_refills_refills_sum:
   apply (case_tac list; clarsimp simp: add_ac)
   done
 
+method refill_head_overlapping_loop_simple
+  = ((clarsimp simp: refill_head_overlapping_loop_def)?
+     , wpsimp wp: whileLoop_wp' set_refills_wp get_refills_wp
+            simp: merge_refills_def round_robin_def refill_pop_head_def sc_valid_refills_def
+                  update_sched_context_set_refills_rewrite update_refill_hd_rewrite
+                  vs_all_heap_simps obj_at_def)
+
 lemma refill_head_overlapping_loop_refills_sum:
-  "refill_head_overlapping_loop sc_ptr
+  "refill_head_overlapping_loop sc_ptr'
    \<lbrace>\<lambda>s. pred_map (\<lambda>cfg. refills_sum (scrc_refills cfg) = scrc_budget cfg)
                  (sc_refill_cfgs_of s) sc_ptr\<rbrace>"
   apply (clarsimp simp: refill_head_overlapping_loop_def)
+  apply (cases "sc_ptr'\<noteq>sc_ptr")
+   apply refill_head_overlapping_loop_simple
   apply (wpsimp wp: whileLoop_wp'; fastforce?)
   apply (wpsimp wp: merge_refills_refills_sum)
   apply (fastforce intro!: refill_head_overlapping_true_imp_length_at_least_two
                      simp: vs_all_heap_simps)
+
   done
 
 lemma merge_refills_refills_unat_sum:
   "\<lbrace>\<lambda>s. pred_map (\<lambda>cfg. refills_unat_sum (scrc_refills cfg) \<le> unat max_time)
-                 (sc_refill_cfgs_of s) sc_ptr
-        \<and> pred_map (\<lambda>cfg. 1 < length (scrc_refills cfg)) (sc_refill_cfgs_of s) sc_ptr\<rbrace>
-   merge_refills sc_ptr
+                      (sc_refill_cfgs_of s) sc_ptr
+        \<and> (sc_ptr' = sc_ptr \<longrightarrow>  pred_map (\<lambda>cfg. 1 < length (scrc_refills cfg))
+                                          (sc_refill_cfgs_of s) sc_ptr)\<rbrace>
+   merge_refills sc_ptr'
    \<lbrace>\<lambda>_ s. pred_map (\<lambda>cfg. refills_unat_sum (scrc_refills cfg) \<le> unat max_time)
                    (sc_refill_cfgs_of s) sc_ptr\<rbrace>"
   apply merge_refills_simple
@@ -7084,19 +7096,22 @@ lemma merge_refills_refills_unat_sum:
 
 lemma merge_refills_hd_r_time:
   "\<lbrace>\<lambda>s. pred_map (\<lambda>cfg. r_time (scrc_refill_hd cfg) \<le> P (cur_time s))
-                 (sc_refill_cfgs_of s) sc_ptr
-        \<and> pred_map (\<lambda>cfg. Suc 0 < length (scrc_refills cfg)) (sc_refill_cfgs_of s) sc_ptr\<rbrace>
-   merge_refills sc_ptr
+                   (sc_refill_cfgs_of s) sc_ptr
+        \<and> (sc_ptr' = sc_ptr \<longrightarrow> pred_map (\<lambda>cfg. Suc 0 < length (scrc_refills cfg))
+                                         (sc_refill_cfgs_of s) sc_ptr)\<rbrace>
+   merge_refills sc_ptr'
    \<lbrace>\<lambda>_ s. pred_map (\<lambda>cfg. r_time (scrc_refill_hd cfg) \<le> P (cur_time s))
                    (sc_refill_cfgs_of s) sc_ptr\<rbrace>"
   apply merge_refills_simple
   done
 
 lemma refill_head_overlapping_loop_hd_r_time:
-  "refill_head_overlapping_loop sc_ptr
+  "refill_head_overlapping_loop sc_ptr'
    \<lbrace>\<lambda>s. pred_map (\<lambda>cfg. r_time (hd (scrc_refills cfg)) \<le> P (cur_time s))
                  (sc_refill_cfgs_of s) sc_ptr\<rbrace>"
   apply (clarsimp simp: refill_head_overlapping_loop_def)
+  apply (cases "sc_ptr'\<noteq>sc_ptr")
+   apply refill_head_overlapping_loop_simple
   apply (wpsimp wp: whileLoop_wp'; fastforce?)
   apply (wpsimp wp: merge_refills_hd_r_time)
   apply (fastforce intro!: refill_head_overlapping_true_imp_length_at_least_two
@@ -7105,19 +7120,22 @@ lemma refill_head_overlapping_loop_hd_r_time:
 
 lemma merge_refills_hd_r_time_unat:
   "\<lbrace>\<lambda>s. pred_map (\<lambda>cfg. unat (r_time (scrc_refill_hd cfg)) \<le> P (cur_time s))
-                 (sc_refill_cfgs_of s) sc_ptr
-        \<and> pred_map (\<lambda>cfg. Suc 0 < length (scrc_refills cfg)) (sc_refill_cfgs_of s) sc_ptr\<rbrace>
-   merge_refills sc_ptr
+                      (sc_refill_cfgs_of s) sc_ptr
+        \<and> (sc_ptr' = sc_ptr \<longrightarrow> pred_map (\<lambda>cfg. Suc 0 < length (scrc_refills cfg))
+                                         (sc_refill_cfgs_of s) sc_ptr)\<rbrace>
+   merge_refills sc_ptr'
    \<lbrace>\<lambda>_ s. pred_map (\<lambda>cfg. unat (r_time (scrc_refill_hd cfg)) \<le> P (cur_time s))
                    (sc_refill_cfgs_of s) sc_ptr\<rbrace>"
   apply merge_refills_simple
   done
 
 lemma refill_head_overlapping_loop_hd_r_time_unat:
-  "refill_head_overlapping_loop sc_ptr
+  "refill_head_overlapping_loop sc_ptr'
    \<lbrace>\<lambda>s. pred_map (\<lambda>cfg. unat (r_time (hd (scrc_refills cfg))) \<le> P (cur_time s))
-                             (sc_refill_cfgs_of s) sc_ptr\<rbrace>"
+                              (sc_refill_cfgs_of s) sc_ptr\<rbrace>"
   apply (clarsimp simp: refill_head_overlapping_loop_def)
+  apply (cases "sc_ptr'\<noteq>sc_ptr")
+   apply refill_head_overlapping_loop_simple
   apply (wpsimp wp: whileLoop_wp'; fastforce?)
   apply (wpsimp wp: merge_refills_hd_r_time_unat)
   apply (fastforce intro!: refill_head_overlapping_true_imp_length_at_least_two
@@ -7125,13 +7143,13 @@ lemma refill_head_overlapping_loop_hd_r_time_unat:
   done
 
 lemma merge_refills_is_refill_ready:
-  "merge_refills sc_ptr \<lbrace>is_refill_ready sc_ptr'\<rbrace>"
+  "merge_refills sc_ptr' \<lbrace>is_refill_ready sc_ptr\<rbrace>"
   apply merge_refills_simple
   apply (clarsimp simp: refill_ready_def)
   done
 
 lemma refill_head_overlapping_is_refill_ready:
-  "refill_head_overlapping_loop sc_ptr \<lbrace>is_refill_ready sc_ptr'\<rbrace>"
+  "refill_head_overlapping_loop sc_ptr' \<lbrace>is_refill_ready sc_ptr\<rbrace>"
   apply (clarsimp simp: refill_head_overlapping_loop_def)
   apply (wpsimp wp: whileLoop_wp'; fastforce?)
   apply (wpsimp wp: merge_refills_is_refill_ready)
@@ -7139,10 +7157,11 @@ lemma refill_head_overlapping_is_refill_ready:
 
 lemma merge_refills_hd_r_amount:
   "\<lbrace>\<lambda>s. pred_map (\<lambda>cfg. a \<le> r_amount (scrc_refill_hd cfg)) (sc_refill_cfgs_of s) sc_ptr
-        \<and> pred_map (\<lambda>cfg. refills_unat_sum (scrc_refills cfg) \<le> unat max_time)
-                    (sc_refill_cfgs_of s) sc_ptr
-        \<and> pred_map (\<lambda>cfg. Suc 0 < length (scrc_refills cfg)) (sc_refill_cfgs_of s) sc_ptr\<rbrace>
-   merge_refills sc_ptr
+        \<and> (sc_ptr' = sc_ptr
+            \<longrightarrow> pred_map (\<lambda>cfg. refills_unat_sum (scrc_refills cfg) \<le> unat max_time)
+                         (sc_refill_cfgs_of s) sc_ptr
+                \<and> pred_map (\<lambda>cfg. Suc 0 < length (scrc_refills cfg)) (sc_refill_cfgs_of s) sc_ptr)\<rbrace>
+   merge_refills sc_ptr'
    \<lbrace>\<lambda>_ s. pred_map (\<lambda>cfg. a \<le> r_amount (scrc_refill_hd cfg)) (sc_refill_cfgs_of s) sc_ptr\<rbrace>"
   apply merge_refills_simple
   apply (clarsimp simp: refills_unat_sum_def pred_map_simps)
@@ -7160,12 +7179,14 @@ lemma merge_refills_hd_r_amount:
 
 lemma refill_head_overlapping_loop_hd_r_amount:
   "\<lbrace>\<lambda>s. pred_map (\<lambda>cfg. a \<le> r_amount (hd (scrc_refills cfg))) (sc_refill_cfgs_of s) sc_ptr
-        \<and> pred_map (\<lambda>cfg. refills_unat_sum (scrc_refills cfg) \<le> unat max_time)
-                    (sc_refill_cfgs_of s) sc_ptr\<rbrace>
-   refill_head_overlapping_loop sc_ptr
+        \<and> (sc_ptr' = sc_ptr \<longrightarrow> pred_map (\<lambda>cfg. refills_unat_sum (scrc_refills cfg) \<le> unat max_time)
+                                         (sc_refill_cfgs_of s) sc_ptr)\<rbrace>
+   refill_head_overlapping_loop sc_ptr'
    \<lbrace>\<lambda>_ s. pred_map (\<lambda>cfg. a \<le> r_amount (hd (scrc_refills cfg))) (sc_refill_cfgs_of s) sc_ptr\<rbrace>"
   (is "valid ?pre _ _")
   apply (clarsimp simp: refill_head_overlapping_loop_def)
+  apply (cases "sc_ptr' \<noteq> sc_ptr")
+   apply refill_head_overlapping_loop_simple
   apply (wpsimp wp: valid_whileLoop[where I="\<lambda>_. ?pre"]; fastforce?)
   apply (intro hoare_vcg_conj_lift_pre_fix)
    apply (wpsimp wp: merge_refills_hd_r_amount)
@@ -7178,10 +7199,11 @@ lemma refill_head_overlapping_loop_hd_r_amount:
 
 lemma merge_refills_no_overflow_helper:
   "\<lbrace>\<lambda>s. pred_map (\<lambda>cfg. unat (r_time (scrc_refill_hd cfg)) + refills_unat_sum (scrc_refills cfg)
-                        \<le> unat max_time)
-                 (sc_refill_cfgs_of s) sc_ptr
-        \<and> pred_map (\<lambda>cfg. Suc 0 < length (scrc_refills cfg)) (sc_refill_cfgs_of s) sc_ptr\<rbrace>
-   merge_refills sc_ptr
+                          \<le> unat max_time)
+                   (sc_refill_cfgs_of s) sc_ptr
+        \<and> (sc_ptr' = sc_ptr \<longrightarrow> pred_map (\<lambda>cfg. Suc 0 < length (scrc_refills cfg))
+                                         (sc_refill_cfgs_of s) sc_ptr)\<rbrace>
+   merge_refills sc_ptr'
    \<lbrace>\<lambda>_ s. pred_map (\<lambda>cfg. unat (r_time (scrc_refill_hd cfg)) + refills_unat_sum (scrc_refills cfg)
                           \<le> unat max_time)
                    (sc_refill_cfgs_of s) sc_ptr\<rbrace>"
@@ -7197,11 +7219,12 @@ lemma merge_refills_no_overflow_helper:
 
 lemma merge_refills_no_overflow:
   "\<lbrace>\<lambda>s. pred_map (\<lambda>cfg. no_overflow (scrc_refills cfg)) (sc_refill_cfgs_of s) sc_ptr
-        \<and> pred_map (\<lambda>cfg. unat (r_time (scrc_refill_hd cfg)) + refills_unat_sum (scrc_refills cfg)
-                           \<le> unat max_time)
-                   (sc_refill_cfgs_of s) sc_ptr
-        \<and> pred_map (\<lambda>cfg. Suc 0 < length (scrc_refills cfg)) (sc_refill_cfgs_of s) sc_ptr\<rbrace>
-   merge_refills sc_ptr
+        \<and> (sc_ptr' = sc_ptr
+           \<longrightarrow> pred_map (\<lambda>cfg. unat (r_time (scrc_refill_hd cfg)) + refills_unat_sum (scrc_refills cfg)
+                                \<le> unat max_time)
+                        (sc_refill_cfgs_of s) sc_ptr
+               \<and> pred_map (\<lambda>cfg. Suc 0 < length (scrc_refills cfg)) (sc_refill_cfgs_of s) sc_ptr)\<rbrace>
+   merge_refills sc_ptr'
    \<lbrace>\<lambda>_ s. pred_map (\<lambda>cfg. no_overflow (scrc_refills cfg)) (sc_refill_cfgs_of s) sc_ptr\<rbrace>"
   apply merge_refills_simple
   apply (clarsimp simp: obj_at_def refills_unat_sum_def pred_map_simps)
@@ -7225,13 +7248,16 @@ lemma merge_refills_no_overflow:
 
 lemma refill_head_overlapping_loop_no_overflow:
   "\<lbrace>\<lambda>s. pred_map (\<lambda>cfg. no_overflow (scrc_refills cfg)) (sc_refill_cfgs_of s) sc_ptr
-        \<and> pred_map (\<lambda>cfg. unat (r_time (hd (scrc_refills cfg)))
-                           + refills_unat_sum (scrc_refills cfg) \<le> unat max_time)
-                    (sc_refill_cfgs_of s) sc_ptr\<rbrace>
-   refill_head_overlapping_loop sc_ptr
-   \<lbrace>\<lambda>r s. pred_map (\<lambda>cfg. no_overflow (scrc_refills cfg)) (sc_refill_cfgs_of s) sc_ptr\<rbrace>"
+        \<and> (sc_ptr' = sc_ptr
+           \<longrightarrow> pred_map (\<lambda>cfg. unat (r_time (hd (scrc_refills cfg)))
+                               + refills_unat_sum (scrc_refills cfg) \<le> unat max_time)
+                        (sc_refill_cfgs_of s) sc_ptr)\<rbrace>
+   refill_head_overlapping_loop sc_ptr'
+   \<lbrace>\<lambda>_ s. pred_map (\<lambda>cfg. no_overflow (scrc_refills cfg)) (sc_refill_cfgs_of s) sc_ptr\<rbrace>"
   (is "valid ?pre _ _")
   apply (clarsimp simp: refill_head_overlapping_loop_def)
+  apply (cases "sc_ptr' \<noteq> sc_ptr")
+   apply refill_head_overlapping_loop_simple
   apply (wpsimp wp: valid_whileLoop[where I="\<lambda>_. ?pre"]
          ; fastforce?)
   apply (wpsimp wp: merge_refills_no_overflow_helper merge_refills_no_overflow)
@@ -7241,9 +7267,9 @@ lemma refill_head_overlapping_loop_no_overflow:
 
 lemma merge_refills_ordered_disjoint:
   "\<lbrace>\<lambda>s. pred_map (\<lambda>cfg. ordered_disjoint (scrc_refills cfg)) (sc_refill_cfgs_of s) sc_ptr
-        \<and> pred_map (\<lambda>cfg. refills_unat_sum (scrc_refills cfg) \<le> unat max_time)
-                    (sc_refill_cfgs_of s) sc_ptr\<rbrace>
-   merge_refills sc_ptr
+        \<and> (sc_ptr' = sc_ptr \<longrightarrow> pred_map (\<lambda>cfg. refills_unat_sum (scrc_refills cfg) \<le> unat max_time)
+                                         (sc_refill_cfgs_of s) sc_ptr)\<rbrace>
+   merge_refills sc_ptr'
    \<lbrace>\<lambda>_ s. pred_map (\<lambda>cfg. ordered_disjoint (scrc_refills cfg)) (sc_refill_cfgs_of s) sc_ptr\<rbrace>"
   apply merge_refills_simple
   apply (rename_tac sc n)
@@ -7277,12 +7303,14 @@ lemma merge_refills_ordered_disjoint:
 
 lemma refill_head_overlapping_loop_ordered_disjoint:
   "\<lbrace>\<lambda>s. pred_map (\<lambda>cfg. ordered_disjoint (scrc_refills cfg)) (sc_refill_cfgs_of s) sc_ptr
-        \<and> pred_map (\<lambda>cfg. refills_unat_sum (scrc_refills cfg) \<le> unat max_time)
-                    (sc_refill_cfgs_of s) sc_ptr\<rbrace>
-   refill_head_overlapping_loop sc_ptr
+        \<and> (sc_ptr' = sc_ptr \<longrightarrow> pred_map (\<lambda>cfg. refills_unat_sum (scrc_refills cfg) \<le> unat max_time)
+                                         (sc_refill_cfgs_of s) sc_ptr)\<rbrace>
+   refill_head_overlapping_loop sc_ptr'
    \<lbrace>\<lambda>_ s. pred_map (\<lambda>cfg. ordered_disjoint (scrc_refills cfg)) (sc_refill_cfgs_of s) sc_ptr\<rbrace>"
   (is "valid ?pre _ _")
   apply (clarsimp simp: refill_head_overlapping_loop_def)
+  apply (cases "sc_ptr' \<noteq> sc_ptr")
+   apply refill_head_overlapping_loop_simple
   apply (wpsimp wp: valid_whileLoop[where I="\<lambda>_. ?pre"]
          ; fastforce?)
   apply (wpsimp wp: merge_refills_refills_unat_sum merge_refills_ordered_disjoint)
@@ -7291,16 +7319,20 @@ lemma refill_head_overlapping_loop_ordered_disjoint:
   done
 
 lemma refill_head_overlapping_loop_ordered_disjoint_strong:
-  "\<lbrace>\<lambda>s. pred_map (\<lambda>cfg. ordered_disjoint (tl (scrc_refills cfg))) (sc_refill_cfgs_of s) sc_ptr
-        \<and> pred_map (\<lambda>cfg. no_overflow (scrc_refills cfg)) (sc_refill_cfgs_of s) sc_ptr
-        \<and> pred_map (\<lambda>cfg. unat (r_time (scrc_refill_hd cfg)) + refills_unat_sum (scrc_refills cfg)
-                           \<le> unat max_time)
-                    (sc_refill_cfgs_of s) sc_ptr
-        \<and> pred_map (\<lambda>cfg. refills_unat_sum (scrc_refills cfg) \<le> unat max_time)
-                    (sc_refill_cfgs_of s) sc_ptr\<rbrace>
-   refill_head_overlapping_loop sc_ptr
+  "\<lbrace>\<lambda>s. if sc_ptr' = sc_ptr
+        then pred_map (\<lambda>cfg. ordered_disjoint (tl (scrc_refills cfg))) (sc_refill_cfgs_of s) sc_ptr
+             \<and> pred_map (\<lambda>cfg. no_overflow (scrc_refills cfg)) (sc_refill_cfgs_of s) sc_ptr
+             \<and> pred_map (\<lambda>cfg. unat (r_time (scrc_refill_hd cfg)) + refills_unat_sum (scrc_refills cfg)
+                                \<le> unat max_time)
+                         (sc_refill_cfgs_of s) sc_ptr
+             \<and> pred_map (\<lambda>cfg. refills_unat_sum (scrc_refills cfg) \<le> unat max_time)
+                         (sc_refill_cfgs_of s) sc_ptr
+        else pred_map (\<lambda>cfg. ordered_disjoint (scrc_refills cfg)) (sc_refill_cfgs_of s) sc_ptr\<rbrace>
+   refill_head_overlapping_loop sc_ptr'
    \<lbrace>\<lambda>_ s. pred_map (\<lambda>cfg. ordered_disjoint (scrc_refills cfg)) (sc_refill_cfgs_of s) sc_ptr\<rbrace>"
   (is "valid ?pre _ _")
+  apply (case_tac "sc_ptr' \<noteq> sc_ptr")
+   apply refill_head_overlapping_loop_simple
   apply (clarsimp simp: refill_head_overlapping_loop_def)
   apply (wpsimp wp: valid_whileLoop[where I="\<lambda>_. ?pre", rotated 3]
          ; fastforce?)
@@ -7351,10 +7383,11 @@ lemma refill_head_overlapping_loop_ordered_disjoint_strong:
 
 lemma refill_head_overlapping_loop_window:
   "\<lbrace>\<lambda>s. pred_map (\<lambda>cfg. window (scrc_refills cfg) (scrc_period cfg)) (sc_refill_cfgs_of s) sc_ptr
-        \<and> pred_map (\<lambda>cfg. unat (r_time (hd (scrc_refills cfg)))
-                           + refills_unat_sum (scrc_refills cfg) \<le> unat max_time)
-                    (sc_refill_cfgs_of s) sc_ptr\<rbrace>
-   refill_head_overlapping_loop sc_ptr
+        \<and> (sc_ptr' = sc_ptr
+           \<longrightarrow>  pred_map (\<lambda>cfg. unat (r_time (hd (scrc_refills cfg)))
+                                 + refills_unat_sum (scrc_refills cfg) \<le> unat max_time)
+                         (sc_refill_cfgs_of s) sc_ptr)\<rbrace>
+   refill_head_overlapping_loop sc_ptr'
    \<lbrace>\<lambda>_ s. pred_map (\<lambda>cfg. window (scrc_refills cfg) (scrc_period cfg)) (sc_refill_cfgs_of s) sc_ptr\<rbrace>"
   apply (clarsimp simp: refill_head_overlapping_loop_def)
   apply (wpsimp wp: whileLoop_wp'; fastforce?)
@@ -7363,7 +7396,7 @@ lemma refill_head_overlapping_loop_window:
   done
 
 lemma refill_head_overlapping_loop_length:
-  "refill_head_overlapping_loop sc_ptr
+  "refill_head_overlapping_loop sc_ptr'
    \<lbrace>\<lambda>s. pred_map (\<lambda>cfg. length (scrc_refills cfg) \<le> scrc_refill_max cfg) (sc_refill_cfgs_of s) sc_ptr\<rbrace>"
   apply (clarsimp simp: refill_head_overlapping_loop_def)
   apply (wpsimp wp: whileLoop_wp'; fastforce?)
@@ -7418,16 +7451,14 @@ method non_overlapping_merge_refills_simple
      , (clarsimp simp: vs_all_heap_simps obj_at_def)?)
 
 lemma non_overlapping_merge_refills_nonempty_refills:
-  "\<lbrace>\<lambda>s. pred_map (\<lambda>cfg. scrc_refills cfg \<noteq> []) (sc_refill_cfgs_of s) sc_ptr \<and> sc_ptr = cur_sc s\<rbrace>
-   non_overlapping_merge_refills sc_ptr
-   \<lbrace>\<lambda>_ s. pred_map (\<lambda>cfg. scrc_refills cfg \<noteq> []) (sc_refill_cfgs_of s) sc_ptr\<rbrace>"
+  "non_overlapping_merge_refills sc_ptr'
+   \<lbrace>\<lambda>s. pred_map (\<lambda>cfg. scrc_refills cfg \<noteq> []) (sc_refill_cfgs_of s) sc_ptr\<rbrace>"
   apply non_overlapping_merge_refills_simple
   done
 
 lemma head_insufficient_loop_nonempty_refills:
-  "\<lbrace>\<lambda>s. pred_map (\<lambda>cfg. scrc_refills cfg \<noteq> []) (sc_refill_cfgs_of s) sc_ptr \<and> sc_ptr = cur_sc s\<rbrace>
-   head_insufficient_loop sc_ptr
-   \<lbrace>\<lambda>_ s. pred_map (\<lambda>cfg. scrc_refills cfg \<noteq> []) (sc_refill_cfgs_of s) sc_ptr\<rbrace>"
+  "head_insufficient_loop sc_ptr'
+   \<lbrace>\<lambda>s. pred_map (\<lambda>cfg. scrc_refills cfg \<noteq> []) (sc_refill_cfgs_of s) sc_ptr\<rbrace>"
   (is "valid ?pre _ _")
   apply (clarsimp simp: head_insufficient_loop_def)
   apply (wpsimp wp: valid_whileLoop[where I="\<lambda>_. ?pre"]; fastforce?)
@@ -7450,9 +7481,10 @@ lemma head_insufficient_length_at_least_two:
 
 lemma non_overlapping_merge_refills_refills_unat_sum:
   "\<lbrace>\<lambda>s. pred_map (\<lambda>cfg. refills_unat_sum (scrc_refills cfg) \<le> unat max_time)
-                 (sc_refill_cfgs_of s) sc_ptr
-        \<and> pred_map (\<lambda>cfg. 1 < length (scrc_refills cfg)) (sc_refill_cfgs_of s) sc_ptr\<rbrace>
-   non_overlapping_merge_refills sc_ptr
+                      (sc_refill_cfgs_of s) sc_ptr
+        \<and> (sc_ptr' = sc_ptr \<longrightarrow> pred_map (\<lambda>cfg. 1 < length (scrc_refills cfg))
+                                         (sc_refill_cfgs_of s) sc_ptr)\<rbrace>
+   non_overlapping_merge_refills sc_ptr'
    \<lbrace>\<lambda>_ s. pred_map (\<lambda>cfg. refills_unat_sum (scrc_refills cfg) \<le> unat max_time)
                    (sc_refill_cfgs_of s) sc_ptr\<rbrace>"
   apply non_overlapping_merge_refills_simple
@@ -7469,11 +7501,12 @@ lemma non_overlapping_merge_refills_refills_unat_sum:
 
 lemma non_overlapping_merge_refills_refills_unat_sum_lower_bound:
   "\<lbrace>\<lambda>s. pred_map (\<lambda>cfg. unat MIN_BUDGET \<le> refills_unat_sum (scrc_refills cfg))
-                 (sc_refill_cfgs_of s) sc_ptr
-        \<and> pred_map (\<lambda>cfg. refills_unat_sum (scrc_refills cfg) \<le> unat max_time)
-                    (sc_refill_cfgs_of s) sc_ptr
-        \<and> pred_map (\<lambda>cfg. 1 < length (scrc_refills cfg)) (sc_refill_cfgs_of s) sc_ptr\<rbrace>
-   non_overlapping_merge_refills sc_ptr
+                      (sc_refill_cfgs_of s) sc_ptr
+        \<and> (sc_ptr' = sc_ptr
+           \<longrightarrow> pred_map (\<lambda>cfg. refills_unat_sum (scrc_refills cfg) \<le> unat max_time)
+                        (sc_refill_cfgs_of s) sc_ptr
+               \<and> pred_map (\<lambda>cfg. 1 < length (scrc_refills cfg)) (sc_refill_cfgs_of s) sc_ptr)\<rbrace>
+   non_overlapping_merge_refills sc_ptr'
    \<lbrace>\<lambda>_ s. pred_map (\<lambda>cfg. unat MIN_BUDGET \<le> refills_unat_sum (scrc_refills cfg))
                    (sc_refill_cfgs_of s) sc_ptr\<rbrace>"
   apply non_overlapping_merge_refills_simple
@@ -7487,17 +7520,30 @@ lemma non_overlapping_merge_refills_refills_unat_sum_lower_bound:
   apply (case_tac list; clarsimp)
   done
 
+method head_insufficient_loop_simple
+  = ((clarsimp simp: head_insufficient_loop_def)?
+     , wpsimp wp: whileLoop_wp' set_refills_wp get_refills_wp
+            simp: non_overlapping_merge_refills_def refill_pop_head_def schedule_used_defs
+                  update_sched_context_set_refills_rewrite update_refill_hd_rewrite
+     , clarsimp simp: vs_all_heap_simps obj_at_def sc_valid_refills_def round_robin_def
+                      unat_MAX_RELEASE_TIME
+               split: if_splits
+     , fastforce?)
+
 lemma head_insufficient_loop_refills_sum:
   "\<lbrace>\<lambda>s. pred_map (\<lambda>cfg. refills_sum (scrc_refills cfg) = scrc_budget cfg)
-                 (sc_refill_cfgs_of s) sc_ptr
-        \<and> pred_map (\<lambda>cfg. unat MIN_BUDGET \<le> refills_unat_sum (scrc_refills cfg))
-                    (sc_refill_cfgs_of s) sc_ptr
-        \<and> pred_map (\<lambda>cfg. refills_unat_sum (scrc_refills cfg) \<le> unat max_time)
-                    (sc_refill_cfgs_of s) sc_ptr \<and> sc_ptr = cur_sc s\<rbrace>
-   head_insufficient_loop sc_ptr
+                      (sc_refill_cfgs_of s) sc_ptr
+        \<and> (sc_ptr' = sc_ptr
+           \<longrightarrow> pred_map (\<lambda>cfg. unat MIN_BUDGET \<le> refills_unat_sum (scrc_refills cfg))
+                        (sc_refill_cfgs_of s) sc_ptr
+               \<and> pred_map (\<lambda>cfg. refills_unat_sum (scrc_refills cfg) \<le> unat max_time)
+                         (sc_refill_cfgs_of s) sc_ptr)\<rbrace>
+   head_insufficient_loop sc_ptr'
    \<lbrace>\<lambda>_ s. pred_map (\<lambda>cfg. refills_sum (scrc_refills cfg) = scrc_budget cfg)
                    (sc_refill_cfgs_of s) sc_ptr\<rbrace>"
   (is "valid ?pre _ _")
+  apply (cases "sc_ptr' \<noteq> sc_ptr")
+   apply head_insufficient_loop_simple
   apply (clarsimp simp: head_insufficient_loop_def)
   apply (wpsimp wp: valid_whileLoop[where I="\<lambda>_. ?pre"]
          ; fastforce?)
@@ -7521,11 +7567,12 @@ lemma head_insufficient_loop_refills_sum:
 
 lemma non_overlapping_merge_refills_refills_unat_sum_equals_budget:
   "\<lbrace>\<lambda>s. pred_map (\<lambda>cfg. refills_unat_sum (scrc_refills cfg) = unat (scrc_budget cfg))
-                 (sc_refill_cfgs_of s) sc_ptr
-        \<and> pred_map (\<lambda>cfg. refills_unat_sum (scrc_refills cfg) \<le> unat max_time)
-                    (sc_refill_cfgs_of s) sc_ptr
-        \<and> pred_map (\<lambda>cfg. 1 < length (scrc_refills cfg)) (sc_refill_cfgs_of s) sc_ptr\<rbrace>
-   non_overlapping_merge_refills sc_ptr
+                      (sc_refill_cfgs_of s) sc_ptr
+        \<and> (sc_ptr' = sc_ptr
+           \<longrightarrow> pred_map (\<lambda>cfg. refills_unat_sum (scrc_refills cfg) \<le> unat max_time)
+                        (sc_refill_cfgs_of s) sc_ptr
+               \<and> pred_map (\<lambda>cfg. 1 < length (scrc_refills cfg)) (sc_refill_cfgs_of s) sc_ptr)\<rbrace>
+   non_overlapping_merge_refills sc_ptr'
    \<lbrace>\<lambda>_ s. pred_map (\<lambda>cfg. refills_unat_sum (scrc_refills cfg) = unat (scrc_budget cfg))
                    (sc_refill_cfgs_of s) sc_ptr\<rbrace>"
   apply non_overlapping_merge_refills_simple
@@ -7543,16 +7590,18 @@ lemma non_overlapping_merge_refills_refills_unat_sum_equals_budget:
 
 lemma head_insufficient_loop_refills_unat_sum_equals_budget:
   "\<lbrace>\<lambda>s. pred_map (\<lambda>cfg. refills_unat_sum (scrc_refills cfg) = unat (scrc_budget cfg))
-                 (sc_refill_cfgs_of s) sc_ptr
-        \<and> pred_map (\<lambda>cfg. refills_unat_sum (scrc_refills cfg) \<le> unat max_time)
-                    (sc_refill_cfgs_of s) sc_ptr
-        \<and> pred_map (\<lambda>cfg. unat MIN_BUDGET \<le> refills_unat_sum (scrc_refills cfg))
-                    (sc_refill_cfgs_of s) sc_ptr
-        \<and> sc_ptr = cur_sc s\<rbrace>
-   head_insufficient_loop sc_ptr
+                      (sc_refill_cfgs_of s) sc_ptr
+        \<and> (sc_ptr' = sc_ptr
+           \<longrightarrow> pred_map (\<lambda>cfg. refills_unat_sum (scrc_refills cfg) \<le> unat max_time)
+                        (sc_refill_cfgs_of s) sc_ptr
+               \<and> pred_map (\<lambda>cfg. unat MIN_BUDGET \<le> refills_unat_sum (scrc_refills cfg))
+                          (sc_refill_cfgs_of s) sc_ptr)\<rbrace>
+   head_insufficient_loop sc_ptr'
    \<lbrace>\<lambda>_ s. pred_map (\<lambda>cfg. refills_unat_sum (scrc_refills cfg) = unat (scrc_budget cfg))
                    (sc_refill_cfgs_of s) sc_ptr\<rbrace>"
   (is "valid ?pre _ _")
+  apply (cases "sc_ptr' \<noteq> sc_ptr")
+   apply head_insufficient_loop_simple
   apply (clarsimp simp: head_insufficient_loop_def)
   apply (wpsimp wp: valid_whileLoop[where I="\<lambda>_. ?pre"]
          ; fastforce?)
@@ -7601,11 +7650,10 @@ lemma non_overlapping_merge_refills_ordered_disjoint_helper:
 
 lemma non_overlapping_merge_refills_ordered_disjoint:
   "\<lbrace>\<lambda>s. pred_map (\<lambda>cfg. ordered_disjoint (scrc_refills cfg))
-                 (sc_refill_cfgs_of s) sc_ptr
-        \<and> pred_map (\<lambda>cfg. refills_unat_sum (scrc_refills cfg) \<le> unat max_time)
-                    (sc_refill_cfgs_of s) sc_ptr
-        \<and> sc_ptr = cur_sc s\<rbrace>
-   non_overlapping_merge_refills sc_ptr
+                      (sc_refill_cfgs_of s) sc_ptr
+        \<and> (sc_ptr' = sc_ptr \<longrightarrow> pred_map (\<lambda>cfg. refills_unat_sum (scrc_refills cfg) \<le> unat max_time)
+                                         (sc_refill_cfgs_of s) sc_ptr)\<rbrace>
+   non_overlapping_merge_refills sc_ptr'
    \<lbrace>\<lambda>_ s. pred_map (\<lambda>cfg. ordered_disjoint (scrc_refills cfg)) (sc_refill_cfgs_of s) sc_ptr\<rbrace>"
   apply non_overlapping_merge_refills_simple
   apply (clarsimp simp: refills_unat_sum_def)
@@ -7619,14 +7667,16 @@ lemma non_overlapping_merge_refills_ordered_disjoint:
 
 lemma head_insufficient_loop_ordered_disjoint:
   "\<lbrace>\<lambda>s. pred_map (\<lambda>cfg. ordered_disjoint (scrc_refills cfg)) (sc_refill_cfgs_of s) sc_ptr
-        \<and> pred_map (\<lambda>cfg. unat MIN_BUDGET \<le> refills_unat_sum (scrc_refills cfg))
-                    (sc_refill_cfgs_of s) sc_ptr
-        \<and> pred_map (\<lambda>cfg. refills_unat_sum (scrc_refills cfg) \<le> unat max_time)
-                    (sc_refill_cfgs_of s) sc_ptr
-        \<and> sc_ptr = cur_sc s\<rbrace>
-   head_insufficient_loop sc_ptr
+        \<and> (sc_ptr' = sc_ptr
+           \<longrightarrow> pred_map (\<lambda>cfg. unat MIN_BUDGET \<le> refills_unat_sum (scrc_refills cfg))
+                        (sc_refill_cfgs_of s) sc_ptr
+               \<and> pred_map (\<lambda>cfg. refills_unat_sum (scrc_refills cfg) \<le> unat max_time)
+                          (sc_refill_cfgs_of s) sc_ptr)\<rbrace>
+   head_insufficient_loop sc_ptr'
    \<lbrace>\<lambda>_ s. pred_map (\<lambda>cfg. ordered_disjoint (scrc_refills cfg)) (sc_refill_cfgs_of s) sc_ptr\<rbrace>"
   (is "valid ?pre _ _")
+  apply (cases "sc_ptr' \<noteq> sc_ptr")
+   apply head_insufficient_loop_simple
   apply (clarsimp simp: head_insufficient_loop_def)
   apply (wpsimp wp: valid_whileLoop[where I="\<lambda>_. ?pre"]
          ; fastforce?)
@@ -7678,11 +7728,11 @@ lemma non_overlapping_merge_refills_no_overflow_helper:
 
 lemma non_overlapping_merge_refills_no_overflow:
   "\<lbrace>\<lambda>s. pred_map (\<lambda>cfg. no_overflow (scrc_refills cfg)) (sc_refill_cfgs_of s) sc_ptr
-        \<and> pred_map (\<lambda>cfg. ordered_disjoint (scrc_refills cfg))
-                    (sc_refill_cfgs_of s) sc_ptr
-        \<and> pred_map (\<lambda>cfg. 1 < length (scrc_refills cfg)) (sc_refill_cfgs_of s) sc_ptr
-        \<and> sc_ptr = cur_sc s\<rbrace>
-   non_overlapping_merge_refills sc_ptr
+        \<and> (sc_ptr' = sc_ptr
+           \<longrightarrow> pred_map (\<lambda>cfg. ordered_disjoint (scrc_refills cfg))
+                        (sc_refill_cfgs_of s) sc_ptr
+               \<and> pred_map (\<lambda>cfg. 1 < length (scrc_refills cfg)) (sc_refill_cfgs_of s) sc_ptr)\<rbrace>
+   non_overlapping_merge_refills sc_ptr'
    \<lbrace>\<lambda>_ s. pred_map (\<lambda>cfg. no_overflow (scrc_refills cfg)) (sc_refill_cfgs_of s) sc_ptr\<rbrace>"
   apply non_overlapping_merge_refills_simple
   apply (rename_tac sc n)
@@ -7695,15 +7745,17 @@ lemma non_overlapping_merge_refills_no_overflow:
 
 lemma head_insufficient_loop_no_overflow:
   "\<lbrace>\<lambda>s. pred_map (\<lambda>cfg. no_overflow (scrc_refills cfg)) (sc_refill_cfgs_of s) sc_ptr
-        \<and> pred_map (\<lambda>cfg. ordered_disjoint (scrc_refills cfg)) (sc_refill_cfgs_of s) sc_ptr
-        \<and> pred_map (\<lambda>cfg. unat MIN_BUDGET \<le> refills_unat_sum (scrc_refills cfg))
-                    (sc_refill_cfgs_of s) sc_ptr
-        \<and> pred_map (\<lambda>cfg. refills_unat_sum (scrc_refills cfg) \<le> unat max_time)
-                    (sc_refill_cfgs_of s) sc_ptr
-        \<and> sc_ptr = cur_sc s\<rbrace>
-   head_insufficient_loop sc_ptr
+        \<and> (sc_ptr' = sc_ptr
+           \<longrightarrow> pred_map (\<lambda>cfg. ordered_disjoint (scrc_refills cfg)) (sc_refill_cfgs_of s) sc_ptr
+               \<and> pred_map (\<lambda>cfg. unat MIN_BUDGET \<le> refills_unat_sum (scrc_refills cfg))
+                          (sc_refill_cfgs_of s) sc_ptr
+               \<and> pred_map (\<lambda>cfg. refills_unat_sum (scrc_refills cfg) \<le> unat max_time)
+                          (sc_refill_cfgs_of s) sc_ptr)\<rbrace>
+   head_insufficient_loop sc_ptr'
    \<lbrace>\<lambda>_ s. pred_map (\<lambda>cfg. no_overflow (scrc_refills cfg)) (sc_refill_cfgs_of s) sc_ptr\<rbrace>"
   (is "valid ?pre _ _")
+  apply (cases "sc_ptr' \<noteq> sc_ptr")
+   apply head_insufficient_loop_simple
   apply (clarsimp simp: head_insufficient_loop_def)
   apply (wpsimp wp: valid_whileLoop[where I="\<lambda>_. ?pre"]
          ; fastforce?)
@@ -7720,16 +7772,18 @@ lemma head_insufficient_loop_no_overflow:
 
 lemma head_insufficient_loop_refills_window:
   "\<lbrace>\<lambda>s. pred_map (\<lambda>cfg. window (scrc_refills cfg) (scrc_period cfg)) (sc_refill_cfgs_of s) sc_ptr
-        \<and> pred_map (\<lambda>cfg. ordered_disjoint (scrc_refills cfg))
-                    (sc_refill_cfgs_of s) sc_ptr
-        \<and> pred_map (\<lambda>cfg. unat MIN_BUDGET \<le> refills_unat_sum (scrc_refills cfg))
-                    (sc_refill_cfgs_of s) sc_ptr
-        \<and> pred_map (\<lambda>cfg. refills_unat_sum (scrc_refills cfg) \<le> unat max_time)
-                    (sc_refill_cfgs_of s) sc_ptr
-        \<and> sc_ptr = cur_sc s\<rbrace>
-   head_insufficient_loop sc_ptr
+        \<and> (sc_ptr' = sc_ptr
+           \<longrightarrow>  pred_map (\<lambda>cfg. ordered_disjoint (scrc_refills cfg))
+                         (sc_refill_cfgs_of s) sc_ptr
+               \<and> pred_map (\<lambda>cfg. unat MIN_BUDGET \<le> refills_unat_sum (scrc_refills cfg))
+                          (sc_refill_cfgs_of s) sc_ptr
+               \<and> pred_map (\<lambda>cfg. refills_unat_sum (scrc_refills cfg) \<le> unat max_time)
+                          (sc_refill_cfgs_of s) sc_ptr)\<rbrace>
+   head_insufficient_loop sc_ptr'
    \<lbrace>\<lambda>_ s. pred_map (\<lambda>cfg. window (scrc_refills cfg) (scrc_period cfg)) (sc_refill_cfgs_of s) sc_ptr\<rbrace>"
   (is "valid ?pre _ _")
+  apply (cases "sc_ptr' \<noteq> sc_ptr")
+   apply head_insufficient_loop_simple
   apply (clarsimp simp: head_insufficient_loop_def)
   apply (wpsimp wp: valid_whileLoop[where I="\<lambda>_. ?pre"]
          ; fastforce?)
@@ -7759,20 +7813,24 @@ lemma head_insufficient_loop_refills_window:
   done
 
 lemma head_insufficient_loop_hd_r_time:
-  "\<lbrace>\<lambda>s. pred_map (\<lambda>cfg. unat (r_time (last (scrc_refills cfg))) \<le> P (cur_time s))
-                 (sc_refill_cfgs_of s) sc_ptr
-        \<and> pred_map (\<lambda>cfg. ordered_disjoint (scrc_refills cfg)) (sc_refill_cfgs_of s) sc_ptr
-        \<and> pred_map (\<lambda>cfg. no_overflow (scrc_refills cfg)) (sc_refill_cfgs_of s) sc_ptr
-        \<and> pred_map (\<lambda>cfg. refills_unat_sum (scrc_refills cfg) \<le> unat max_time)
-                    (sc_refill_cfgs_of s) sc_ptr
-        \<and> pred_map (\<lambda>cfg. unat MIN_BUDGET \<le> refills_unat_sum (scrc_refills cfg))
-                    (sc_refill_cfgs_of s) sc_ptr
-        \<and> pred_map (\<lambda>cfg. scrc_refills cfg \<noteq> []) (sc_refill_cfgs_of s) sc_ptr
-        \<and> sc_ptr = cur_sc s\<rbrace>
-   head_insufficient_loop sc_ptr
+  "\<lbrace>\<lambda>s. if sc_ptr' = sc_ptr
+        then pred_map (\<lambda>cfg. unat (r_time (last (scrc_refills cfg))) \<le> P (cur_time s))
+                      (sc_refill_cfgs_of s) sc_ptr
+             \<and> pred_map (\<lambda>cfg. ordered_disjoint (scrc_refills cfg)) (sc_refill_cfgs_of s) sc_ptr
+             \<and> pred_map (\<lambda>cfg. no_overflow (scrc_refills cfg)) (sc_refill_cfgs_of s) sc_ptr
+             \<and> pred_map (\<lambda>cfg. refills_unat_sum (scrc_refills cfg) \<le> unat max_time)
+                         (sc_refill_cfgs_of s) sc_ptr
+             \<and> pred_map (\<lambda>cfg. unat MIN_BUDGET \<le> refills_unat_sum (scrc_refills cfg))
+                         (sc_refill_cfgs_of s) sc_ptr
+             \<and> pred_map (\<lambda>cfg. scrc_refills cfg \<noteq> []) (sc_refill_cfgs_of s) sc_ptr
+        else pred_map (\<lambda>cfg. unat (r_time (hd (scrc_refills cfg))) \<le> P (cur_time s))
+                   (sc_refill_cfgs_of s) sc_ptr\<rbrace>
+   head_insufficient_loop sc_ptr'
    \<lbrace>\<lambda>_ s. pred_map (\<lambda>cfg. unat (r_time (hd (scrc_refills cfg))) \<le> P (cur_time s))
                    (sc_refill_cfgs_of s) sc_ptr\<rbrace>"
   (is "valid ?pre _ _")
+  apply (cases "sc_ptr' \<noteq> sc_ptr")
+   apply head_insufficient_loop_simple
   apply (clarsimp simp: head_insufficient_loop_def)
   apply (wpsimp wp: valid_whileLoop[where I="\<lambda>_. ?pre"]
          ; fastforce?)
@@ -7804,8 +7862,8 @@ lemma head_insufficient_loop_hd_r_time:
     apply (clarsimp simp: word_le_nat_alt ordered_disjoint_def)
     apply (drule_tac x=0 in spec)
     apply clarsimp
-    apply (metis Groups.add_ac(2) One_nat_def Suc_diff_Suc ab_semigroup_add_class.add_ac(1)
-                 hd_conv_nth le_iff_add length_ineq_not_Nil(1) length_tl nth_tl zero_less_Suc)
+    subgoal by (metis Groups.add_ac(2) One_nat_def Suc_diff_Suc ab_semigroup_add_class.add_ac(1)
+                      hd_conv_nth le_iff_add length_ineq_not_Nil(1) length_tl nth_tl zero_less_Suc)
    apply (rename_tac sc n)
    apply (rule_tac y="unat (r_time (hd (tl (sc_refills sc))))" in order_trans
           ; fastforce?)
@@ -7818,14 +7876,15 @@ lemma head_insufficient_loop_hd_r_time:
 
 lemma head_insufficient_loop_hd_r_time_same:
   "\<lbrace>\<lambda>s. pred_map (\<lambda>cfg. r_time (hd (scrc_refills cfg)) \<le> P (cur_time s))
-                 (sc_refill_cfgs_of s) sc_ptr
-        \<and> pred_map (\<lambda>cfg. MIN_BUDGET \<le> r_amount (hd (scrc_refills cfg)))
-                    (sc_refill_cfgs_of s) sc_ptr
-        \<and> sc_ptr = cur_sc s\<rbrace>
-   head_insufficient_loop sc_ptr
+                      (sc_refill_cfgs_of s) sc_ptr
+        \<and> (sc_ptr' = sc_ptr \<longrightarrow>  pred_map (\<lambda>cfg. MIN_BUDGET \<le> r_amount (hd (scrc_refills cfg)))
+                                          (sc_refill_cfgs_of s) sc_ptr)\<rbrace>
+   head_insufficient_loop sc_ptr'
    \<lbrace>\<lambda>_ s. pred_map (\<lambda>cfg. r_time (hd (scrc_refills cfg)) \<le> P (cur_time s))
                    (sc_refill_cfgs_of s) sc_ptr\<rbrace>"
   (is "valid ?pre _ _")
+  apply (cases "sc_ptr' \<noteq> sc_ptr")
+   apply head_insufficient_loop_simple
   apply (clarsimp simp: head_insufficient_loop_def)
   apply (wpsimp wp: valid_whileLoop[where I="\<lambda>_. ?pre"]
          ; fastforce?)
@@ -7836,16 +7895,20 @@ lemma head_insufficient_loop_hd_r_time_same:
   done
 
 lemma head_insufficient_loop_MIN_BUDGET_in_head:
-  "\<lbrace>\<lambda>s. pred_map (\<lambda>cfg. refills_unat_sum (scrc_refills cfg) \<le> unat max_time)
+  "\<lbrace>\<lambda>s. if sc_ptr' = sc_ptr
+        then pred_map (\<lambda>cfg. refills_unat_sum (scrc_refills cfg) \<le> unat max_time)
+                      (sc_refill_cfgs_of s) sc_ptr
+             \<and> pred_map (\<lambda>cfg. unat MIN_BUDGET \<le> refills_unat_sum (scrc_refills cfg))
                          (sc_refill_cfgs_of s) sc_ptr
-        \<and> pred_map (\<lambda>cfg. unat MIN_BUDGET \<le> refills_unat_sum (scrc_refills cfg))
-                    (sc_refill_cfgs_of s) sc_ptr
-        \<and> pred_map (\<lambda>cfg. scrc_refills cfg \<noteq> []) (sc_refill_cfgs_of s) sc_ptr
-        \<and> sc_ptr = cur_sc s\<rbrace>
-   head_insufficient_loop sc_ptr
+             \<and> pred_map (\<lambda>cfg. scrc_refills cfg \<noteq> []) (sc_refill_cfgs_of s) sc_ptr
+        else pred_map (\<lambda>cfg. MIN_BUDGET \<le> r_amount (hd (scrc_refills cfg)))
+                   (sc_refill_cfgs_of s) sc_ptr\<rbrace>
+   head_insufficient_loop sc_ptr'
    \<lbrace>\<lambda>_ s. pred_map (\<lambda>cfg. MIN_BUDGET \<le> r_amount (hd (scrc_refills cfg)))
                    (sc_refill_cfgs_of s) sc_ptr\<rbrace>"
   (is "valid ?pre _ _")
+  apply (cases "sc_ptr' \<noteq> sc_ptr")
+   apply head_insufficient_loop_simple
   apply (clarsimp simp: head_insufficient_loop_def)
   apply (wpsimp wp: valid_whileLoop[where I="\<lambda>_. ?pre"]
          ; fastforce?)
@@ -7861,10 +7924,10 @@ lemma head_insufficient_loop_MIN_BUDGET_in_head:
 
 lemma non_overlapping_merge_refills_length_bounded:
   "\<lbrace>\<lambda>s. pred_map (\<lambda>cfg. length (scrc_refills cfg) \<le> scrc_refill_max cfg)
-                 (sc_refill_cfgs_of s) sc_ptr
-        \<and> pred_map (\<lambda>cfg. 1 < length (scrc_refills cfg)) (sc_refill_cfgs_of s) sc_ptr
-        \<and> sc_ptr = cur_sc s\<rbrace>
-   non_overlapping_merge_refills sc_ptr
+                      (sc_refill_cfgs_of s) sc_ptr
+        \<and> (sc_ptr' = sc_ptr \<longrightarrow>  pred_map (\<lambda>cfg. 1 < length (scrc_refills cfg))
+                                          (sc_refill_cfgs_of s) sc_ptr)\<rbrace>
+   non_overlapping_merge_refills sc_ptr'
    \<lbrace>\<lambda>_ s. pred_map (\<lambda>cfg. length (scrc_refills cfg) \<le> scrc_refill_max cfg)
                    (sc_refill_cfgs_of s) sc_ptr\<rbrace>"
   apply non_overlapping_merge_refills_simple
@@ -7873,16 +7936,18 @@ lemma non_overlapping_merge_refills_length_bounded:
 
 lemma head_insufficient_loop_length_bounded:
   "\<lbrace>\<lambda>s. pred_map (\<lambda>cfg. length (scrc_refills cfg) \<le> scrc_refill_max cfg)
-                 (sc_refill_cfgs_of s) sc_ptr
-        \<and> pred_map (\<lambda>cfg. unat MIN_BUDGET \<le> refills_unat_sum (scrc_refills cfg))
-                    (sc_refill_cfgs_of s) sc_ptr
-        \<and> pred_map (\<lambda>cfg. refills_unat_sum (scrc_refills cfg) \<le> unat max_time)
-                    (sc_refill_cfgs_of s) sc_ptr
-        \<and> sc_ptr = cur_sc s\<rbrace>
-   head_insufficient_loop sc_ptr
+                      (sc_refill_cfgs_of s) sc_ptr
+        \<and> (sc_ptr' = sc_ptr
+           \<longrightarrow>  pred_map (\<lambda>cfg. unat MIN_BUDGET \<le> refills_unat_sum (scrc_refills cfg))
+                         (sc_refill_cfgs_of s) sc_ptr
+               \<and> pred_map (\<lambda>cfg. refills_unat_sum (scrc_refills cfg) \<le> unat max_time)
+                           (sc_refill_cfgs_of s) sc_ptr)\<rbrace>
+   head_insufficient_loop sc_ptr'
    \<lbrace>\<lambda>_ s. pred_map (\<lambda>cfg. length (scrc_refills cfg) \<le> scrc_refill_max cfg)
                    (sc_refill_cfgs_of s) sc_ptr\<rbrace>"
   (is "valid ?pre _ _")
+  apply (cases "sc_ptr' \<noteq> sc_ptr")
+   apply head_insufficient_loop_simple
   apply (clarsimp simp: head_insufficient_loop_def)
   apply (wpsimp wp: valid_whileLoop[where I="\<lambda>_. ?pre"]
          ; fastforce?)
@@ -7909,7 +7974,9 @@ abbreviation sp_valid_refills_unbundled where
    \<and> pred_map (\<lambda>cfg. MIN_BUDGET \<le> scrc_budget cfg) (sc_refill_cfgs_of s) sc_ptr
    \<and> pred_map (\<lambda>cfg. scrc_budget cfg \<le> scrc_period cfg) (sc_refill_cfgs_of s) sc_ptr
    \<and> pred_map (\<lambda>cfg. MIN_REFILLS \<le> scrc_refill_max cfg) (sc_refill_cfgs_of s) sc_ptr
-   \<and> pred_map (\<lambda>cfg. scrc_period cfg \<le> MAX_PERIOD) (sc_refill_cfgs_of s) sc_ptr"
+   \<and> pred_map (\<lambda>cfg. scrc_period cfg \<le> MAX_PERIOD) (sc_refill_cfgs_of s) sc_ptr
+   \<and> pred_map (\<lambda>cfg. \<forall>refill \<in> set (scrc_refills cfg). 0 < unat (r_amount refill))
+               (sc_refill_cfgs_of s) sc_ptr"
 
 lemma valid_refills_unbundled:
   "\<lbrakk>\<not> round_robin sc_ptr s; sp_valid_refills_unbundled sc_ptr s\<rbrakk> \<Longrightarrow> valid_refills sc_ptr s"
@@ -8064,7 +8131,9 @@ lemma refill_new_valid_refills[wp]:
          clarsimp simp: refills_sum_def obj_at_def MIN_REFILLS_def vs_all_heap_simps
                         ordered_disjoint_def no_overflow_def
                         window_def sc_valid_refills_def rr_valid_refills_def split: if_splits)
-  apply (fastforce simp: word_le_nat_alt)
+  apply (insert MIN_BUDGET_pos)
+  apply (clarsimp simp: word_le_nat_alt)
+  apply (metis linorder_not_le unat_gt_0 word_less_nat_alt)
   done
 
 lemma refill_update_valid_refills:
@@ -8080,6 +8149,7 @@ lemma refill_update_valid_refills:
    refill_update p new_period new_budget new_max_refills
    \<lbrace>\<lambda>_. valid_refills scptr\<rbrace>"
   supply if_split [split del]
+  apply (insert MIN_BUDGET_pos)
   unfolding refill_update_def maybe_add_empty_tail_def refill_add_tail_def update_refill_tl_def
             update_refill_hd_def
   apply (wpsimp wp: set_refills_wp update_sched_context_wp is_round_robin_wp get_refills_wp)
@@ -8103,44 +8173,56 @@ lemma refill_update_valid_refills:
    apply (clarsimp simp: valid_refills_def no_overflow_def window_def MIN_REFILLS_def)
    apply (intro conjI)
     apply (clarsimp simp: word_le_nat_alt)
+    apply (metis linorder_not_le unat_gt_0 word_less_nat_alt)
    apply (clarsimp simp: valid_refills_def rr_valid_refills_def no_overflow_def window_def
                          MIN_REFILLS_def)
    apply (intro conjI impI)
-      apply (fastforce elim: word_plus_mono_right2 intro: unat_sum_boundE unat_le_mono)
-     apply (fastforce simp: word_le_nat_alt)
-    apply (subst unat_sub)
-     apply fastforce
-    apply (fastforce simp: word_le_nat_alt)
-   apply presburger
+        apply (fastforce elim: word_plus_mono_right2 intro: unat_sum_boundE unat_le_mono)
+       apply (fastforce simp: word_le_nat_alt)
+      apply (fastforce simp: word_le_nat_alt unat_sub)
+     apply presburger
+    apply (clarsimp simp: word_le_nat_alt word_less_nat_alt split: if_splits)
+   apply (fastforce simp: word_le_nat_alt unat_sub)
 
   \<comment> \<open>scptr is not refill_ready\<close>
+
   apply (rename_tac sc n)
+  apply (insert MIN_BUDGET_pos)
   apply (intro conjI; intro allI impI)
    apply (fastforce simp: valid_refills_def no_overflow_def window_def MIN_REFILLS_def
-                          word_le_nat_alt)
+                          word_le_nat_alt word_less_nat_alt)
   apply (clarsimp simp: valid_refills_def rr_valid_refills_def no_overflow_def window_def
                         MIN_REFILLS_def)
   apply (intro conjI)
+        apply (subst unat_add_lem')
+         apply (clarsimp simp: max_word_def)
+        apply (meson add_le_cancel_left linorder_not_less order_trans word_le_less_eq
+                     word_less_nat_alt)
+       apply (fastforce simp: word_le_nat_alt)
+      apply (subst unat_sub; fastforce?)
       apply (subst unat_add_lem')
        apply (clarsimp simp: max_word_def)
-      apply (meson add_le_cancel_left linorder_not_less order_trans word_le_less_eq
-                   word_less_nat_alt)
-     apply (fastforce simp: word_le_nat_alt)
-    apply (subst unat_sub; fastforce?)
-    apply (subst unat_add_lem')
-     apply (clarsimp simp: max_word_def)
-    apply (prop_tac "unat new_budget - unat (r_amount (refill_hd sc)) \<le> unat new_period")
-     using diff_le_self le_trans unat_le_mono apply blast
-    apply fastforce
-   using unat_plus_gt apply blast
-  apply presburger
+      apply (prop_tac "unat new_budget - unat (r_amount (refill_hd sc)) \<le> unat new_period")
+       using diff_le_self le_trans unat_le_mono apply blast
+      apply fastforce
+     using unat_plus_gt apply blast
+    apply presburger
+   apply (clarsimp simp: word_le_nat_alt word_less_nat_alt split: if_splits)
+  apply (fastforce simp: word_le_nat_alt unat_sub)
   done
 
+method schedule_used_simple
+  = (wpsimp wp: set_refills_wp get_refills_wp
+          simp: update_refill_hd_rewrite update_sched_context_set_refills_rewrite schedule_used_defs
+     , clarsimp simp: round_robin_def vs_all_heap_simps obj_at_def sc_valid_refills_def)
+
 lemma schedule_used_sum:
-  "\<lbrace>\<lambda>s. pred_map (\<lambda>cfg. refills_sum ((scrc_refills cfg) @ [new]) = t) (sc_refill_cfgs_of s) (cur_sc s)
-        \<and> sc_ptr = cur_sc s\<rbrace>
-   schedule_used sc_ptr new
-   \<lbrace>\<lambda>_ s. pred_map (\<lambda>cfg. refills_sum (scrc_refills cfg) = t) (sc_refill_cfgs_of s) (cur_sc s)\<rbrace>"
+  "\<lbrace>\<lambda>s. if sc_ptr' = sc_ptr
+        then pred_map (\<lambda>cfg. refills_sum ((scrc_refills cfg) @ [new]) = t)
+                      (sc_refill_cfgs_of s) sc_ptr
+        else pred_map (\<lambda>cfg. refills_sum (scrc_refills cfg) = t) (sc_refill_cfgs_of s) sc_ptr\<rbrace>
+   schedule_used sc_ptr' new
+   \<lbrace>\<lambda>_ s. pred_map (\<lambda>cfg. refills_sum (scrc_refills cfg) = t) (sc_refill_cfgs_of s) sc_ptr\<rbrace>"
   apply (wpsimp wp: update_sched_context_wp get_refills_wp
               simp: schedule_used_def refill_add_tail_def update_refill_tl_def)
   apply (rename_tac sc n)
@@ -8223,14 +8305,15 @@ lemma valid_refills_r_amount_bounded_max_sc_period:
   done
 
 lemma schedule_used_release_time_bounded:
-  "\<lbrace>\<lambda>s. pred_map (\<lambda>cfg. scrc_refills cfg \<noteq> [] \<longrightarrow> r_time (scrc_refill_hd cfg) \<le> r_time new)
-                 (sc_refill_cfgs_of s) (cur_sc s)
-        \<and> pred_map (\<lambda>cfg. scrc_refills cfg \<noteq> [] \<longrightarrow> r_time new - r_amount (scrc_refill_hd cfg)
-                                                      \<le> r_time new)
-                   (sc_refill_cfgs_of s) (cur_sc s)
-        \<and> sc_ptr = cur_sc s\<rbrace>
-   schedule_used sc_ptr new
-   \<lbrace>\<lambda>_ s. pred_map (\<lambda>cfg. r_time (scrc_refill_hd cfg) \<le> r_time new) (sc_refill_cfgs_of s) (cur_sc s)\<rbrace>"
+  "\<lbrace>\<lambda>s. if sc_ptr' = sc_ptr
+        then pred_map (\<lambda>cfg. scrc_refills cfg \<noteq> [] \<longrightarrow> r_time (scrc_refill_hd cfg) \<le> r_time new)
+                      (sc_refill_cfgs_of s) sc_ptr
+             \<and> pred_map (\<lambda>cfg. scrc_refills cfg \<noteq> [] \<longrightarrow> r_time new - r_amount (scrc_refill_hd cfg)
+                                                           \<le> r_time new)
+                        (sc_refill_cfgs_of s) sc_ptr
+        else pred_map (\<lambda>cfg. r_time (scrc_refill_hd cfg) \<le> r_time new) (sc_refill_cfgs_of s) sc_ptr\<rbrace>
+   schedule_used sc_ptr' new
+   \<lbrace>\<lambda>_ s. pred_map (\<lambda>cfg. r_time (scrc_refill_hd cfg) \<le> r_time new) (sc_refill_cfgs_of s) sc_ptr\<rbrace>"
   apply (wpsimp wp: update_sched_context_wp get_refills_wp
               simp: schedule_used_defs)
   apply (clarsimp simp: obj_at_def vs_all_heap_simps)
@@ -8238,15 +8321,18 @@ lemma schedule_used_release_time_bounded:
   done
 
 lemma schedule_used_refills_unat_sum:
-  "\<lbrace>\<lambda>s. pred_map (\<lambda>cfg. refills_unat_sum ((scrc_refills cfg) @ [new]) = unat (scrc_budget cfg))
-                 (sc_refill_cfgs_of s) (cur_sc s)
-        \<and> sc_ptr = cur_sc s\<rbrace>
-   schedule_used sc_ptr new
+  "\<lbrace>\<lambda>s. if sc_ptr' = sc_ptr
+        then pred_map (\<lambda>cfg. refills_unat_sum ((scrc_refills cfg) @ [new]) = unat (scrc_budget cfg))
+                 (sc_refill_cfgs_of s) sc_ptr
+        else pred_map (\<lambda>cfg. refills_unat_sum (scrc_refills cfg) = unat (scrc_budget cfg))
+                      (sc_refill_cfgs_of s) sc_ptr\<rbrace>
+   schedule_used sc_ptr' new
    \<lbrace>\<lambda>_ s. pred_map (\<lambda>cfg. refills_unat_sum (scrc_refills cfg) = unat (scrc_budget cfg))
-                   (sc_refill_cfgs_of s) (cur_sc s)\<rbrace>"
+                   (sc_refill_cfgs_of s) sc_ptr\<rbrace>"
   supply map_map[simp del]
   apply (wpsimp wp: update_sched_context_wp get_refills_wp
               simp: schedule_used_def refill_add_tail_def update_refill_tl_def)
+
   apply (rename_tac sc n)
   apply (clarsimp simp: schedule_used_def vs_all_heap_simps obj_at_def)
   apply (case_tac "can_merge_refill (refill_tl sc) new")
@@ -8304,17 +8390,20 @@ lemma refill_budget_check_refill_amount_helper:
   done
 
 lemma schedule_used_no_overflow:
-  "\<lbrace>\<lambda>s. pred_map (\<lambda>cfg. no_overflow (scrc_refills cfg)) (sc_refill_cfgs_of s) (cur_sc s)
-        \<and> pred_map (\<lambda>cfg. scrc_refills cfg \<noteq> []
-                           \<longrightarrow> unat (r_time (last (scrc_refills cfg)))
-                                + unat (r_amount (last (scrc_refills cfg)))
-                                + unat (r_amount new)
-                               \<le> unat max_time)
-                   (sc_refill_cfgs_of s) (cur_sc s)
-        \<and> no_overflow [new] \<and> sc_ptr = cur_sc s\<rbrace>
-   schedule_used sc_ptr new
-   \<lbrace>\<lambda>_ s. pred_map (\<lambda>cfg. no_overflow (scrc_refills cfg)) (sc_refill_cfgs_of s) (cur_sc s)\<rbrace>"
+  "\<lbrace>\<lambda>s. pred_map (\<lambda>cfg. no_overflow (scrc_refills cfg)) (sc_refill_cfgs_of s) sc_ptr
+        \<and> (sc_ptr' = sc_ptr
+           \<longrightarrow> (pred_map (\<lambda>cfg. scrc_refills cfg \<noteq> []
+                                \<longrightarrow> unat (r_time (last (scrc_refills cfg)))
+                                     + unat (r_amount (last (scrc_refills cfg)))
+                                     + unat (r_amount new)
+                                    \<le> unat max_time)
+                         (sc_refill_cfgs_of s) sc_ptr
+                \<and> no_overflow [new]))\<rbrace>
+   schedule_used sc_ptr' new
+   \<lbrace>\<lambda>_ s. pred_map (\<lambda>cfg. no_overflow (scrc_refills cfg)) (sc_refill_cfgs_of s) sc_ptr\<rbrace>"
   supply map_map[simp del]
+  apply (cases "sc_ptr'\<noteq>sc_ptr")
+   apply schedule_used_simple
   apply (wpsimp wp: update_sched_context_wp get_refills_wp
               simp: schedule_used_def refill_add_tail_def update_refill_tl_def)
   apply (rename_tac sc n)
@@ -8368,14 +8457,16 @@ lemma schedule_used_no_overflow:
   done
 
 lemma schedule_used_ordered_disjoint:
-  "\<lbrace>\<lambda>s. pred_map (\<lambda>cfg. ordered_disjoint (scrc_refills cfg)) (sc_refill_cfgs_of s) (cur_sc s)
-        \<and> pred_map (\<lambda>cfg. no_overflow (scrc_refills cfg)) (sc_refill_cfgs_of s) (cur_sc s)
-        \<and> pred_map (\<lambda>cfg. scrc_refills cfg \<noteq> [] \<longrightarrow> unat (r_time (last (scrc_refills cfg)))
-                                                     \<le> unat (r_time new))
-                   (sc_refill_cfgs_of s) (cur_sc s)
-        \<and> cur_sc s = sc_ptr\<rbrace>
-   schedule_used sc_ptr new
-   \<lbrace>\<lambda>_ s. pred_map (\<lambda>cfg. ordered_disjoint (scrc_refills cfg)) (sc_refill_cfgs_of s) (cur_sc s)\<rbrace>"
+  "\<lbrace>\<lambda>s. pred_map (\<lambda>cfg. ordered_disjoint (scrc_refills cfg)) (sc_refill_cfgs_of s) sc_ptr
+        \<and> (sc_ptr' = sc_ptr
+           \<longrightarrow>  pred_map (\<lambda>cfg. no_overflow (scrc_refills cfg)) (sc_refill_cfgs_of s) sc_ptr
+                \<and> pred_map (\<lambda>cfg. scrc_refills cfg \<noteq> [] \<longrightarrow> unat (r_time (last (scrc_refills cfg)))
+                                                             \<le> unat (r_time new))
+                           (sc_refill_cfgs_of s) sc_ptr)\<rbrace>
+   schedule_used sc_ptr' new
+   \<lbrace>\<lambda>_ s. pred_map (\<lambda>cfg. ordered_disjoint (scrc_refills cfg)) (sc_refill_cfgs_of s) sc_ptr\<rbrace>"
+  apply (cases "sc_ptr'\<noteq>sc_ptr")
+   apply schedule_used_simple
   apply (wpsimp wp: update_sched_context_wp get_refills_wp
               simp: schedule_used_def refill_add_tail_def update_refill_tl_def)
   apply (rename_tac sc n)
@@ -8450,17 +8541,20 @@ lemma schedule_used_ordered_disjoint:
   done
 
 lemma schedule_used_window:
-  "\<lbrace>\<lambda>s. pred_map (\<lambda>cfg. ordered_disjoint (scrc_refills cfg)) (sc_refill_cfgs_of s) (cur_sc s)
-        \<and> pred_map (\<lambda>cfg. window (scrc_refills cfg) (scrc_period cfg)) (sc_refill_cfgs_of s) (cur_sc s)
-        \<and> pred_map (\<lambda>cfg. no_overflow (scrc_refills cfg)) (sc_refill_cfgs_of s) (cur_sc s)
-        \<and> pred_map (\<lambda>cfg. scrc_refills cfg \<noteq> []) (sc_refill_cfgs_of s) (cur_sc s)
-        \<and> pred_map (\<lambda>cfg. r_time new \<le> r_time (scrc_refill_hd cfg) + scrc_period cfg)
-                    (sc_refill_cfgs_of s) (cur_sc s)
-        \<and> pred_map (\<lambda>cfg. unat (r_time (scrc_refill_hd cfg)) +  unat MAX_PERIOD \<le> unat max_time)
-                    (sc_refill_cfgs_of s) (cur_sc s)
-        \<and> pred_map (\<lambda>cfg. scrc_period cfg \<le> MAX_PERIOD) (sc_refill_cfgs_of s) (cur_sc s)\<rbrace>
-   schedule_used sc_ptr new
-   \<lbrace>\<lambda>_ s. pred_map (\<lambda>cfg. window (scrc_refills cfg) (scrc_period cfg)) (sc_refill_cfgs_of s) (cur_sc s)\<rbrace>"
+  "\<lbrace>\<lambda>s. pred_map (\<lambda>cfg. window (scrc_refills cfg) (scrc_period cfg)) (sc_refill_cfgs_of s) sc_ptr
+        \<and> (sc_ptr' = sc_ptr
+           \<longrightarrow> pred_map (\<lambda>cfg. ordered_disjoint (scrc_refills cfg)) (sc_refill_cfgs_of s) sc_ptr
+               \<and> pred_map (\<lambda>cfg. no_overflow (scrc_refills cfg)) (sc_refill_cfgs_of s) sc_ptr
+               \<and> pred_map (\<lambda>cfg. scrc_refills cfg \<noteq> []) (sc_refill_cfgs_of s) sc_ptr
+               \<and> pred_map (\<lambda>cfg. r_time new \<le> r_time (scrc_refill_hd cfg) + scrc_period cfg)
+                          (sc_refill_cfgs_of s) sc_ptr
+               \<and> pred_map (\<lambda>cfg. unat (r_time (scrc_refill_hd cfg)) +  unat MAX_PERIOD \<le> unat max_time)
+                          (sc_refill_cfgs_of s) sc_ptr
+               \<and> pred_map (\<lambda>cfg. scrc_period cfg \<le> MAX_PERIOD) (sc_refill_cfgs_of s) sc_ptr)\<rbrace>
+   schedule_used sc_ptr' new
+   \<lbrace>\<lambda>_ s. pred_map (\<lambda>cfg. window (scrc_refills cfg) (scrc_period cfg)) (sc_refill_cfgs_of s) sc_ptr\<rbrace>"
+  apply (cases "sc_ptr'\<noteq>sc_ptr")
+   apply schedule_used_simple
   apply (wpsimp wp: update_sched_context_wp get_refills_wp
               simp: schedule_used_def refill_add_tail_def update_refill_tl_def)
   apply (rename_tac sc n)
@@ -8518,7 +8612,9 @@ abbreviation all_sp_valid_refills_but_MIN_BUDGET_in_head where
    \<and> pred_map (\<lambda>cfg. MIN_BUDGET \<le> scrc_budget cfg) (sc_refill_cfgs_of s) sc_ptr
    \<and> pred_map (\<lambda>cfg. scrc_budget cfg \<le> scrc_period cfg) (sc_refill_cfgs_of s) sc_ptr
    \<and> pred_map (\<lambda>cfg. MIN_REFILLS \<le> scrc_refill_max cfg) (sc_refill_cfgs_of s) sc_ptr
-   \<and> pred_map (\<lambda>cfg. scrc_period cfg \<le> MAX_PERIOD) (sc_refill_cfgs_of s) sc_ptr"
+   \<and> pred_map (\<lambda>cfg. scrc_period cfg \<le> MAX_PERIOD) (sc_refill_cfgs_of s) sc_ptr
+   \<and> pred_map (\<lambda>cfg. \<forall>refill \<in> set (scrc_refills cfg). 0 < unat (r_amount refill))
+               (sc_refill_cfgs_of s) sc_ptr"
 
 abbreviation all_sp_valid_refills_but_MIN_BUDGET_in_head_no_overflow where
   "all_sp_valid_refills_but_MIN_BUDGET_in_head_no_overflow sc_ptr s \<equiv>
@@ -8530,29 +8626,39 @@ abbreviation all_sp_valid_refills_but_MIN_BUDGET_in_head_no_overflow where
    \<and> pred_map (\<lambda>cfg. MIN_BUDGET \<le> scrc_budget cfg) (sc_refill_cfgs_of s) sc_ptr
    \<and> pred_map (\<lambda>cfg. scrc_budget cfg \<le> scrc_period cfg) (sc_refill_cfgs_of s) sc_ptr
    \<and> pred_map (\<lambda>cfg. MIN_REFILLS \<le> scrc_refill_max cfg) (sc_refill_cfgs_of s) sc_ptr
-   \<and> pred_map (\<lambda>cfg. scrc_period cfg \<le> MAX_PERIOD) (sc_refill_cfgs_of s) sc_ptr"
+   \<and> pred_map (\<lambda>cfg. scrc_period cfg \<le> MAX_PERIOD) (sc_refill_cfgs_of s) sc_ptr
+   \<and> pred_map (\<lambda>cfg. \<forall>refill \<in> set (scrc_refills cfg). 0 < unat (r_amount refill))
+               (sc_refill_cfgs_of s) sc_ptr"
 
 lemma schedule_used_length_max:
-  "\<lbrace>\<lambda>s. pred_map (\<lambda>cfg. l = length (scrc_refills cfg)) (sc_refill_cfgs_of s) (cur_sc s)\<rbrace>
-   schedule_used sc_ptr new
-   \<lbrace>\<lambda>_ s. pred_map (\<lambda>cfg. length (scrc_refills cfg) \<le> Suc l) (sc_refill_cfgs_of s) (cur_sc s)\<rbrace>"
+  "\<lbrace>\<lambda>s. if sc_ptr' = sc_ptr
+        then pred_map (\<lambda>cfg. l = length (scrc_refills cfg)) (sc_refill_cfgs_of s) sc_ptr
+        else pred_map (\<lambda>cfg. length (scrc_refills cfg) \<le> Suc l) (sc_refill_cfgs_of s) sc_ptr\<rbrace>
+   schedule_used sc_ptr' new
+   \<lbrace>\<lambda>_ s. pred_map (\<lambda>cfg. length (scrc_refills cfg) \<le> Suc l) (sc_refill_cfgs_of s) sc_ptr\<rbrace>"
   apply (wpsimp wp: get_refills_wp update_sched_context_wp simp: schedule_used_defs)
   apply (clarsimp simp: vs_all_heap_simps obj_at_def)
   done
 
 lemma head_insufficient_loop_r_time_helper:
   "(n + 1) * unat MAX_PERIOD \<le> unat max_time \<Longrightarrow>
-   \<lbrace>\<lambda>s. all_sp_valid_refills_but_MIN_BUDGET_in_head sc_ptr s
-        \<and> pred_map (\<lambda>cfg. refills_unat_sum (scrc_refills cfg) = unat (scrc_budget cfg))
-                    (sc_refill_cfgs_of s) sc_ptr
-        \<and> pred_map (\<lambda>cfg. unat (r_time (scrc_refill_hd cfg)) + (n + 1) * unat MAX_PERIOD
-                           \<le> unat max_time)
-                    (sc_refill_cfgs_of s) sc_ptr
-        \<and> sc_ptr = cur_sc s\<rbrace>
-   head_insufficient_loop sc_ptr
+   \<lbrace>\<lambda>s. if sc_ptr' = sc_ptr
+        then all_sp_valid_refills_but_MIN_BUDGET_in_head sc_ptr s
+             \<and> pred_map (\<lambda>cfg. refills_unat_sum (scrc_refills cfg) = unat (scrc_budget cfg))
+                         (sc_refill_cfgs_of s) sc_ptr
+             \<and> pred_map (\<lambda>cfg. unat (r_time (scrc_refill_hd cfg)) + (n + 1) * unat MAX_PERIOD
+                                \<le> unat max_time)
+                         (sc_refill_cfgs_of s) sc_ptr
+        else pred_map (\<lambda>cfg. unat (r_time (scrc_refill_hd cfg)) + n * unat MAX_PERIOD
+                             \<le> unat max_time)
+                      (sc_refill_cfgs_of s) sc_ptr\<rbrace>
+   head_insufficient_loop sc_ptr'
    \<lbrace>\<lambda>_ s. pred_map (\<lambda>cfg. unat (r_time (scrc_refill_hd cfg)) + n * unat MAX_PERIOD
                           \<le> unat max_time)
                    (sc_refill_cfgs_of s) sc_ptr\<rbrace>"
+  apply (cases "sc_ptr'\<noteq>sc_ptr")
+   apply head_insufficient_loop_simple
+   apply (clarsimp simp: vs_all_heap_simps)
   apply (rule_tac Q="\<lambda>_ s. pred_map (\<lambda>cfg. unat (r_time (scrc_refill_hd cfg))
                                             \<le> unat max_time - n * unat MAX_PERIOD)
                                     (sc_refill_cfgs_of s) sc_ptr"
@@ -8627,26 +8733,26 @@ method handle_overrun_loop_simple
                   sc_valid_refills_def vs_all_heap_simps obj_at_def refill_budget_check_defs
                   update_sched_context_set_refills_rewrite schedule_used_defs)
 
-lemma handle_overrun_loop_body_nonzero_refills:
+lemma handle_overrun_loop_body_nonzero_refills[wp]:
   "handle_overrun_loop_body usage
-   \<lbrace>\<lambda>s. pred_map (\<lambda>cfg. scrc_refills cfg \<noteq> []) (sc_refill_cfgs_of s) (cur_sc s)\<rbrace>"
+   \<lbrace>\<lambda>s. pred_map (\<lambda>cfg. scrc_refills cfg \<noteq> []) (sc_refill_cfgs_of s) sc_ptr\<rbrace>"
   apply handle_overrun_loop_simple
   done
 
 lemma handle_overrun_loop_nonzero_refills:
   "handle_overrun_loop usage
-   \<lbrace>\<lambda>s. pred_map (\<lambda>cfg. scrc_refills cfg \<noteq> []) (sc_refill_cfgs_of s) (cur_sc s)\<rbrace>"
+   \<lbrace>\<lambda>s. pred_map (\<lambda>cfg. scrc_refills cfg \<noteq> []) (sc_refill_cfgs_of s) sc_ptr\<rbrace>"
   apply (clarsimp simp: handle_overrun_loop_def)
   apply (wpsimp wp: whileLoop_wp' handle_overrun_loop_body_nonzero_refills)
   done
 
 lemma handle_overrun_loop_body_refills_unat_sum_equals_budget:
   "\<lbrace>\<lambda>s. pred_map (\<lambda>cfg. refills_unat_sum (scrc_refills cfg) = unat (scrc_budget cfg))
-                 (sc_refill_cfgs_of s) (cur_sc s)
-        \<and> pred_map (\<lambda>cfg. scrc_refills cfg \<noteq> []) (sc_refill_cfgs_of s) (cur_sc s)\<rbrace>
+                      (sc_refill_cfgs_of s) sc_ptr
+        \<and> (sc_ptr = cur_sc s \<longrightarrow> pred_map (\<lambda>cfg. scrc_refills cfg \<noteq> []) (sc_refill_cfgs_of s) sc_ptr)\<rbrace>
    handle_overrun_loop_body usage
    \<lbrace>\<lambda>_ s. pred_map (\<lambda>cfg. refills_unat_sum (scrc_refills cfg) = unat (scrc_budget cfg))
-                   (sc_refill_cfgs_of s) (cur_sc s)\<rbrace>"
+                   (sc_refill_cfgs_of s) sc_ptr\<rbrace>"
   (is "valid _ _ (\<lambda>_ s. ?post s)")
   supply map_map[simp del]
   apply (clarsimp simp: handle_overrun_loop_body_def)
@@ -8665,35 +8771,36 @@ lemma handle_overrun_loop_body_refills_unat_sum_equals_budget:
                       update_refill_hd_rewrite
                   wp: set_refills_wp get_refills_wp)
   apply (clarsimp simp: vs_all_heap_simps obj_at_def refills_unat_sum_def)
-   apply (rename_tac sc n)
-   apply (case_tac "sc_refills sc"; simp)
+  apply (rename_tac sc n)
+  apply (case_tac "sc_refills sc"; simp)
   done
 
 lemma handle_overrun_loop_refills_unat_sum_equals_budget:
   "\<lbrace>\<lambda>s. pred_map (\<lambda>cfg. refills_unat_sum (scrc_refills cfg) = unat (scrc_budget cfg))
-                 (sc_refill_cfgs_of s) (cur_sc s)
-        \<and> pred_map (\<lambda>cfg. scrc_refills cfg \<noteq> []) (sc_refill_cfgs_of s) (cur_sc s)\<rbrace>
+                      (sc_refill_cfgs_of s) sc_ptr
+        \<and> (sc_ptr = cur_sc s \<longrightarrow>  pred_map (\<lambda>cfg. scrc_refills cfg \<noteq> []) (sc_refill_cfgs_of s) sc_ptr)\<rbrace>
    handle_overrun_loop usage
    \<lbrace>\<lambda>_ s. pred_map (\<lambda>cfg. refills_unat_sum (scrc_refills cfg) = unat (scrc_budget cfg))
-                   (sc_refill_cfgs_of s) (cur_sc s)\<rbrace>"
-  (is "valid ?pre _ _")
+                   (sc_refill_cfgs_of s) sc_ptr\<rbrace>"
+  (is "\<lbrace>?pre\<rbrace> _ \<lbrace>_\<rbrace>")
   apply (clarsimp simp: handle_overrun_loop_def)
   apply (rule_tac I="\<lambda>_. ?pre" in valid_whileLoop; fastforce?)
   apply (wpsimp wp: handle_overrun_loop_body_refills_unat_sum_equals_budget
-                    handle_overrun_loop_body_nonzero_refills)
+                    handle_overrun_loop_body_nonzero_refills hoare_vcg_if_lift2 hoare_vcg_imp_lift')
   done
 
 lemma handle_overrun_loop_body_window:
-  "\<lbrace>\<lambda>s. pred_map (\<lambda>cfg. window (scrc_refills cfg) (scrc_period cfg)) (sc_refill_cfgs_of s) (cur_sc s)
-        \<and> pred_map (\<lambda>cfg. ordered_disjoint (scrc_refills cfg)) (sc_refill_cfgs_of s) (cur_sc s)
-        \<and> pred_map (\<lambda>cfg. no_overflow (scrc_refills cfg)) (sc_refill_cfgs_of s) (cur_sc s)
-        \<and> pred_map (\<lambda>cfg. scrc_refills cfg \<noteq> []) (sc_refill_cfgs_of s) (cur_sc s)
-        \<and> pred_map (\<lambda>cfg. unat (r_time (scrc_refill_hd cfg)) + 2 * unat MAX_PERIOD \<le> unat max_time)
-                   (sc_refill_cfgs_of s) (cur_sc s)
-        \<and> pred_map (\<lambda>cfg. scrc_period cfg \<le> MAX_PERIOD) (sc_refill_cfgs_of s) (cur_sc s)\<rbrace>
+  "\<lbrace>\<lambda>s. pred_map (\<lambda>cfg. window (scrc_refills cfg) (scrc_period cfg)) (sc_refill_cfgs_of s) sc_ptr
+        \<and> (sc_ptr = cur_sc s
+           \<longrightarrow>  pred_map (\<lambda>cfg. ordered_disjoint (scrc_refills cfg)) (sc_refill_cfgs_of s) sc_ptr
+                \<and> pred_map (\<lambda>cfg. no_overflow (scrc_refills cfg)) (sc_refill_cfgs_of s) sc_ptr
+                \<and> pred_map (\<lambda>cfg. scrc_refills cfg \<noteq> []) (sc_refill_cfgs_of s) sc_ptr
+                \<and> pred_map (\<lambda>cfg. unat (r_time (scrc_refill_hd cfg)) + 2 * unat MAX_PERIOD \<le> unat max_time)
+                           (sc_refill_cfgs_of s) sc_ptr
+                \<and> pred_map (\<lambda>cfg. scrc_period cfg \<le> MAX_PERIOD) (sc_refill_cfgs_of s) sc_ptr)\<rbrace>
    handle_overrun_loop_body usage
-   \<lbrace>\<lambda>_ s. pred_map (\<lambda>cfg. window (scrc_refills cfg) (scrc_period cfg)) (sc_refill_cfgs_of s) (cur_sc s)\<rbrace>"
-  (is "valid _ _ (\<lambda>_ s. ?post s)")
+   \<lbrace>\<lambda>_ s. pred_map (\<lambda>cfg. window (scrc_refills cfg) (scrc_period cfg)) (sc_refill_cfgs_of s) sc_ptr\<rbrace>"
+  (is "\<lbrace>_\<rbrace> _ \<lbrace>(\<lambda>_ s. ?post s)\<rbrace>")
   apply (clarsimp simp: handle_overrun_loop_body_def)
   apply (rule hoare_seq_ext[OF _ gets_sp])
   apply (rule hoare_seq_ext[OF _ refill_single_sp])
@@ -8706,6 +8813,8 @@ lemma handle_overrun_loop_body_window:
    apply (simp add: less_not_refl2 tail_nonempty_length)
    apply (wpsimp simp: refill_pop_head_def update_sched_context_set_refills_rewrite
                    wp: schedule_used_window set_refills_wp get_refills_wp)
+  apply (case_tac "sc_ptr \<noteq> cur_sc s")
+   apply (clarsimp simp: vs_all_heap_simps obj_at_def window_def)
   apply (clarsimp simp: vs_all_heap_simps obj_at_def window_def)
   apply (rename_tac sc n)
   apply (prop_tac "unat (r_time (refill_hd sc)) \<le> unat (r_time (hd (tl (sc_refills sc))))")
@@ -8723,11 +8832,10 @@ lemma handle_overrun_loop_body_window:
    apply (rule_tac refills="sc_refills sc" in ordered_disjoint_no_overflow_implies_sorted; simp?)
     apply (simp add: Suc_length_not_empty nat_less_le)
    apply (metis Nitpick.size_list_simp One_nat_def length_tl nat_less_le not_less_eq_eq zero_order)
-  apply (intro conjI impI allI)
-       apply (blast intro: ordered_disjoint_sublist)
-      apply (prop_tac "last (tl (sc_refills sc)) = refill_tl sc")
-       apply (metis Nitpick.size_list_simp last_tl)
-      apply clarsimp
+  apply (prop_tac "last (tl (sc_refills sc)) = refill_tl sc")
+   apply (metis Nitpick.size_list_simp last_tl)
+  apply (intro conjI impI allI; fastforce?)
+      apply (blast intro: ordered_disjoint_sublist)
      apply (blast intro: no_overflow_sublist)
     apply (metis Nitpick.size_list_simp)
    apply (rule word_add_le_mono1)
@@ -8770,21 +8878,28 @@ lemma head_time_buffer_implies_no_overflow:
   done
 
 lemma handle_overrun_loop_body_ordered_disjoint:
-  "\<lbrace>\<lambda>s. pred_map (\<lambda>cfg. ordered_disjoint (scrc_refills cfg)) (sc_refill_cfgs_of s) (cur_sc s)
-        \<and> pred_map (\<lambda>cfg. window (scrc_refills cfg) (scrc_period cfg)) (sc_refill_cfgs_of s) (cur_sc s)
-        \<and> pred_map (\<lambda>cfg. unat (r_time (scrc_refill_hd cfg)) + 2 * unat MAX_PERIOD \<le> unat max_time)
-                   (sc_refill_cfgs_of s) (cur_sc s)
-        \<and> pred_map (\<lambda>cfg. scrc_refills cfg \<noteq> []) (sc_refill_cfgs_of s) (cur_sc s)
-        \<and> pred_map (\<lambda>cfg. scrc_period cfg \<le> MAX_PERIOD) (sc_refill_cfgs_of s) (cur_sc s)
-        \<and> pred_map (\<lambda>cfg. refills_unat_sum (scrc_refills cfg) = unat (scrc_budget cfg))
-                   (sc_refill_cfgs_of s) (cur_sc s)
-        \<and> pred_map (\<lambda>cfg. scrc_budget cfg \<le> scrc_period cfg) (sc_refill_cfgs_of s) (cur_sc s)\<rbrace>
+  "\<lbrace>\<lambda>s. pred_map (\<lambda>cfg. ordered_disjoint (scrc_refills cfg)) (sc_refill_cfgs_of s) sc_ptr
+        \<and> (sc_ptr = cur_sc s
+           \<longrightarrow>  pred_map (\<lambda>cfg. ordered_disjoint (scrc_refills cfg)) (sc_refill_cfgs_of s) sc_ptr
+                \<and> pred_map (\<lambda>cfg. window (scrc_refills cfg) (scrc_period cfg)) (sc_refill_cfgs_of s) sc_ptr
+                \<and> pred_map (\<lambda>cfg. unat (r_time (scrc_refill_hd cfg)) + 2 * unat MAX_PERIOD \<le> unat max_time)
+                           (sc_refill_cfgs_of s) sc_ptr
+                \<and> pred_map (\<lambda>cfg. scrc_refills cfg \<noteq> []) (sc_refill_cfgs_of s) sc_ptr
+                \<and> pred_map (\<lambda>cfg. scrc_period cfg \<le> MAX_PERIOD) (sc_refill_cfgs_of s) sc_ptr
+                \<and> pred_map (\<lambda>cfg. refills_unat_sum (scrc_refills cfg) = unat (scrc_budget cfg))
+                           (sc_refill_cfgs_of s) sc_ptr
+                \<and> pred_map (\<lambda>cfg. scrc_budget cfg \<le> scrc_period cfg) (sc_refill_cfgs_of s) sc_ptr)\<rbrace>
     handle_overrun_loop_body usage
-    \<lbrace>\<lambda>_ s. pred_map (\<lambda>cfg. ordered_disjoint (scrc_refills cfg)) (sc_refill_cfgs_of s) (cur_sc s)\<rbrace>"
+    \<lbrace>\<lambda>_ s. pred_map (\<lambda>cfg. ordered_disjoint (scrc_refills cfg)) (sc_refill_cfgs_of s) sc_ptr\<rbrace>"
   (is "valid _ _ (\<lambda>_ s. ?post s)")
-  apply (rule_tac R1="\<lambda>s. pred_map (\<lambda>cfg. no_overflow (scrc_refills cfg)) (sc_refill_cfgs_of s) (cur_sc s)"
+  apply (rule_tac R1="\<lambda>s. sc_ptr = cur_sc s
+                          \<longrightarrow> pred_map (\<lambda>cfg. no_overflow (scrc_refills cfg))
+                                       (sc_refill_cfgs_of s) (cur_sc s)"
                in hoare_pre_add[THEN iffD2, simplified pred_conj_def])
-   apply (blast intro: head_time_buffer_implies_no_overflow)
+   apply (clarsimp split: if_splits)
+   apply (case_tac "sc_ptr \<noteq> cur_sc s")
+    apply (clarsimp simp: vs_all_heap_simps obj_at_kh_kheap_simps)
+   apply (fastforce intro: head_time_buffer_implies_no_overflow)
   apply (clarsimp simp: handle_overrun_loop_body_def)
   apply (rule hoare_seq_ext[OF _ gets_sp])
   apply (rule hoare_seq_ext[OF _ refill_single_sp])
@@ -8796,6 +8911,8 @@ lemma handle_overrun_loop_body_ordered_disjoint:
    apply (clarsimp simp: vs_all_heap_simps ordered_disjoint_def obj_at_kh_kheap_simps)
   apply (wpsimp simp: refill_pop_head_def update_sched_context_set_refills_rewrite
                   wp: schedule_used_ordered_disjoint set_refills_wp get_refills_wp)
+  apply (case_tac "sc_ptr \<noteq> cur_sc s")
+   apply (clarsimp simp: vs_all_heap_simps obj_at_kh_kheap_simps)
   apply (clarsimp simp: vs_all_heap_simps obj_at_kh_kheap_simps)
   apply (intro conjI impI)
     apply (blast intro: ordered_disjoint_sublist)
@@ -8804,62 +8921,97 @@ lemma handle_overrun_loop_body_ordered_disjoint:
   apply (subst unat_add_lem'; fastforce simp: max_word_def window_def last_tl)
   done
 
+(* FIXME RT: keep? move? *)
+lemma hoare_imp_helper:
+  "\<lbrakk> \<lbrace>P and Q\<rbrace> f \<lbrace>\<lambda>rv s. R rv s\<rbrace>; f \<lbrace>\<lambda>s. \<not> Q s\<rbrace> \<rbrakk> \<Longrightarrow> \<lbrace>\<lambda>s. P s\<rbrace> f \<lbrace>\<lambda>rv s. Q s \<longrightarrow> R rv s\<rbrace>"
+  apply (rule hoare_weaken_pre)
+   apply (rule hoare_vcg_imp_lift')
+    apply fastforce
+   apply fastforce
+  apply (clarsimp simp: pred_conj_def valid_def)
+  done
+
 lemma handle_overrun_loop_ordered_disjoint:
-  "\<lbrace>\<lambda>s. pred_map (\<lambda>cfg. ordered_disjoint (scrc_refills cfg)) (sc_refill_cfgs_of s) (cur_sc s)
-        \<and> pred_map (\<lambda>cfg. window (scrc_refills cfg) (scrc_period cfg)) (sc_refill_cfgs_of s) (cur_sc s)
-        \<and> pred_map (\<lambda>cfg. scrc_refills cfg \<noteq> []) (sc_refill_cfgs_of s) (cur_sc s)
-        \<and> pred_map (\<lambda>cfg. scrc_period cfg \<le> MAX_PERIOD) (sc_refill_cfgs_of s) (cur_sc s)
-        \<and> pred_map (\<lambda>cfg. refills_unat_sum (scrc_refills cfg) = unat (scrc_budget cfg))
-                   (sc_refill_cfgs_of s) (cur_sc s)
-        \<and> pred_map (\<lambda>cfg. scrc_budget cfg \<le> scrc_period cfg) (sc_refill_cfgs_of s) (cur_sc s)\<rbrace>
+  "\<lbrace>\<lambda>s. pred_map (\<lambda>cfg. ordered_disjoint (scrc_refills cfg)) (sc_refill_cfgs_of s) sc_ptr
+        \<and> (sc_ptr = cur_sc s
+           \<longrightarrow> pred_map (\<lambda>cfg. window (scrc_refills cfg) (scrc_period cfg)) (sc_refill_cfgs_of s) sc_ptr
+               \<and> pred_map (\<lambda>cfg. scrc_refills cfg \<noteq> []) (sc_refill_cfgs_of s) sc_ptr
+               \<and> pred_map (\<lambda>cfg. scrc_period cfg \<le> MAX_PERIOD) (sc_refill_cfgs_of s) sc_ptr
+               \<and> pred_map (\<lambda>cfg. refills_unat_sum (scrc_refills cfg) = unat (scrc_budget cfg))
+                          (sc_refill_cfgs_of s) sc_ptr
+               \<and> pred_map (\<lambda>cfg. scrc_budget cfg \<le> scrc_period cfg) (sc_refill_cfgs_of s) sc_ptr)\<rbrace>
    handle_overrun_loop usage
-   \<lbrace>\<lambda>_ s. pred_map (\<lambda>cfg. ordered_disjoint (scrc_refills cfg)) (sc_refill_cfgs_of s) (cur_sc s)\<rbrace>"
+   \<lbrace>\<lambda>_ s. pred_map (\<lambda>cfg. ordered_disjoint (scrc_refills cfg)) (sc_refill_cfgs_of s) sc_ptr\<rbrace>"
   (is "valid ?pre _ _")
+  supply if_split[split del]
   apply (clarsimp simp: handle_overrun_loop_def)
   apply (wpsimp wp: valid_whileLoop[where I="\<lambda>_ s. ?pre s"]
-         ; fastforce?)
-  apply (intro hoare_vcg_conj_lift_pre_fix
-         ; (solves handle_overrun_loop_body_simple)?)
+         ; (fastforce split: if_splits)?)
+  apply (intro hoare_vcg_conj_lift_pre_fix)
     apply (wpsimp wp: handle_overrun_loop_body_ordered_disjoint)
     apply (fastforce dest: head_time_buffer_true_imp_unat_buffer[THEN iffD1, rotated]
                      simp: vs_all_heap_simps unat_MAX_RELEASE_TIME)
-   apply (wpsimp wp: handle_overrun_loop_body_window)
-   apply (fastforce intro!: head_time_buffer_implies_no_overflow
+  apply (rule hoare_imp_helper; (solves handle_overrun_loop_body_simple)?)
+  apply (intro hoare_vcg_conj_lift_pre_fix
+         ; (solves handle_overrun_loop_body_simple)?)
+   apply wpsimp
+   apply (rule_tac f=cur_sc in hoare_lift_Pf2)
+    apply (wpsimp wp: handle_overrun_loop_body_window)
+    apply (fastforce intro!: head_time_buffer_implies_no_overflow
                       dest: head_time_buffer_true_imp_unat_buffer[THEN iffD1, rotated]
                       simp: vs_all_heap_simps unat_MAX_RELEASE_TIME)
-  apply (wpsimp wp: handle_overrun_loop_body_refills_unat_sum_equals_budget)
+   apply wpsimp
+  apply clarsimp
+  apply (rule_tac f=cur_sc in hoare_lift_Pf2)
+   apply (wpsimp wp: handle_overrun_loop_body_refills_unat_sum_equals_budget)
+  apply wpsimp
   done
 
 lemma handle_overrun_loop_window:
-  "\<lbrace>\<lambda>s. pred_map (\<lambda>cfg. window (scrc_refills cfg) (scrc_period cfg)) (sc_refill_cfgs_of s) (cur_sc s)
-        \<and> pred_map (\<lambda>cfg. ordered_disjoint (scrc_refills cfg)) (sc_refill_cfgs_of s)  (cur_sc s)
-        \<and> pred_map (\<lambda>cfg. scrc_refills cfg \<noteq> []) (sc_refill_cfgs_of s)  (cur_sc s)
-        \<and> pred_map (\<lambda>cfg. scrc_period cfg \<le> MAX_PERIOD) (sc_refill_cfgs_of s)  (cur_sc s)
-        \<and> pred_map (\<lambda>cfg. refills_unat_sum (scrc_refills cfg) = unat (scrc_budget cfg))
-                   (sc_refill_cfgs_of s)  (cur_sc s)
-        \<and> pred_map (\<lambda>cfg. scrc_budget cfg \<le> scrc_period cfg) (sc_refill_cfgs_of s)  (cur_sc s)\<rbrace>
+  "\<lbrace>\<lambda>s. pred_map (\<lambda>cfg. window (scrc_refills cfg) (scrc_period cfg))
+                 (sc_refill_cfgs_of s) sc_ptr
+        \<and> (sc_ptr = cur_sc s
+           \<longrightarrow> pred_map (\<lambda>cfg. window (scrc_refills cfg) (scrc_period cfg))
+                        (sc_refill_cfgs_of s) sc_ptr
+               \<and> pred_map (\<lambda>cfg. ordered_disjoint (scrc_refills cfg)) (sc_refill_cfgs_of s) sc_ptr
+               \<and> pred_map (\<lambda>cfg. scrc_refills cfg \<noteq> []) (sc_refill_cfgs_of s) sc_ptr
+               \<and> pred_map (\<lambda>cfg. scrc_period cfg \<le> MAX_PERIOD) (sc_refill_cfgs_of s) sc_ptr
+               \<and> pred_map (\<lambda>cfg. refills_unat_sum (scrc_refills cfg) = unat (scrc_budget cfg))
+                          (sc_refill_cfgs_of s) sc_ptr
+               \<and> pred_map (\<lambda>cfg. scrc_budget cfg \<le> scrc_period cfg) (sc_refill_cfgs_of s) sc_ptr)\<rbrace>
    handle_overrun_loop usage
-   \<lbrace>\<lambda>_ s. pred_map (\<lambda>cfg. window (scrc_refills cfg) (scrc_period cfg)) (sc_refill_cfgs_of s)  (cur_sc s)\<rbrace>"
+   \<lbrace>\<lambda>_ s. pred_map (\<lambda>cfg. window (scrc_refills cfg) (scrc_period cfg)) (sc_refill_cfgs_of s) sc_ptr\<rbrace>"
   (is "valid ?pre _ _")
+  supply if_split[split del]
   apply (clarsimp simp: handle_overrun_loop_def)
   apply (wpsimp wp: valid_whileLoop[where I="\<lambda>_. ?pre"]
          ; fastforce?)
+  apply (rule hoare_vcg_conj_lift_pre_fix)
+   apply (wpsimp wp: handle_overrun_loop_body_window)
+   apply (fastforce intro!: head_time_buffer_implies_no_overflow
+                     dest!: head_time_buffer_true_imp_unat_buffer[THEN iffD1, rotated]
+                      simp: vs_all_heap_simps unat_MAX_RELEASE_TIME)
+  apply (rule hoare_imp_helper; (solves handle_overrun_loop_body_simple)?)
   apply (intro hoare_vcg_conj_lift_pre_fix
          ; (solves handle_overrun_loop_simple)?)
-    apply (wpsimp wp: handle_overrun_loop_body_window)
+    apply (rule hoare_weaken_pre)
+     apply (rule_tac f=cur_sc in hoare_lift_Pf2)
+      apply (wpsimp wp: handle_overrun_loop_body_window)
+     apply wpsimp
     apply (fastforce intro!: head_time_buffer_implies_no_overflow
                       dest!: head_time_buffer_true_imp_unat_buffer[THEN iffD1, rotated]
                        simp: vs_all_heap_simps  unat_MAX_RELEASE_TIME)
-   apply (wpsimp wp: handle_overrun_loop_body_ordered_disjoint)
+   apply (rule hoare_weaken_pre)
+    apply (rule_tac f=cur_sc in hoare_lift_Pf2)
+     apply (wpsimp wp: handle_overrun_loop_body_ordered_disjoint)
+    apply wpsimp
    apply (fastforce dest: head_time_buffer_true_imp_unat_buffer[THEN iffD1, rotated]
                     simp: vs_all_heap_simps MAX_RELEASE_TIME_def MAX_PERIOD_mult' unat_sub)
-  apply (wpsimp wp: handle_overrun_loop_body_refills_unat_sum_equals_budget)
+  apply wpsimp
+  apply (rule_tac f=cur_sc in hoare_lift_Pf2)
+   apply (wpsimp wp: handle_overrun_loop_body_refills_unat_sum_equals_budget)
+  apply wpsimp
   done
-
-method schedule_used_simple
-  = (wpsimp wp: set_refills_wp get_refills_wp
-          simp: update_refill_hd_rewrite update_sched_context_set_refills_rewrite schedule_used_defs
-     , clarsimp simp: round_robin_def vs_all_heap_simps obj_at_def sc_valid_refills_def)
 
 lemma handle_overrun_loop_head_bound:
   "\<lbrace>\<lambda>s. cur_sc_offset_ready 0 s \<and> valid_refills (cur_sc s) s \<and> current_time_bounded 5 s
@@ -8902,27 +9054,36 @@ lemma handle_overrun_loop_head_bound:
   apply (intro hoare_vcg_conj_lift_pre_fix
          ; (solves handle_overrun_loop_body_simple)?)
      defer
-     apply (wpsimp wp: handle_overrun_loop_body_window)
-     apply (fastforce intro!: head_time_buffer_implies_no_overflow
-                        simp: vs_all_heap_simps)
-    apply (wpsimp wp: handle_overrun_loop_body_ordered_disjoint)
-    apply (fastforce simp: vs_all_heap_simps)
-   apply (wpsimp wp: handle_overrun_loop_body_refills_unat_sum_equals_budget)
+     apply (rule_tac f=cur_sc in hoare_lift_Pf2)
+      apply (wpsimp wp: handle_overrun_loop_body_window)
+      apply (fastforce intro!: head_time_buffer_implies_no_overflow
+                         simp: vs_all_heap_simps)
+     apply wpsimp
+    apply (rule_tac f=cur_sc in hoare_lift_Pf2)
+     apply (wpsimp wp: handle_overrun_loop_body_ordered_disjoint)
+     apply (fastforce simp: vs_all_heap_simps)
+    apply wpsimp
+   apply (rule_tac f=cur_sc in hoare_lift_Pf2)
+    apply (wpsimp wp: handle_overrun_loop_body_refills_unat_sum_equals_budget)
+   apply wpsimp
 
-  apply (rule_tac R1="\<lambda>s. pred_map (\<lambda>cfg. no_overflow (scrc_refills cfg)) (sc_refill_cfgs_of s) (cur_sc s)"
+  apply (rule_tac f=cur_sc in hoare_lift_Pf2; (solves wpsimp)?)
+  apply (rename_tac sc_ptr)
+  apply (rule_tac R1="\<lambda>s. pred_map (\<lambda>cfg. no_overflow (scrc_refills cfg)) (sc_refill_cfgs_of s) sc_ptr"
                in hoare_pre_add[THEN iffD2, simplified pred_conj_def])
    apply (fastforce dest!: head_time_buffer_implies_no_overflow[rotated 1]
                      simp: vs_all_heap_simps)
-
   apply (clarsimp simp: handle_overrun_loop_body_def)
   apply (rule hoare_seq_ext[OF _ gets_sp])
   apply (rule hoare_seq_ext[OF _ refill_single_sp])
   apply (rule hoare_seq_ext[OF _ get_sched_context_sp])
-  apply (rule_tac B="\<lambda>_ s. ?post s
+  apply (rule_tac B="\<lambda>_ s. pred_map (\<lambda>cfg. unat (r_time (hd (scrc_refills cfg))) + 4 * unat MAX_PERIOD
+                                            \<le> unat max_time)
+                                    (sc_refill_cfgs_of s) sc_ptr
                            \<and> pred_map (\<lambda>cfg. scrc_period cfg \<le> MAX_PERIOD)
-                                       (sc_refill_cfgs_of s) (cur_sc s)
+                                       (sc_refill_cfgs_of s) sc_ptr
                            \<and> pred_map (\<lambda>cfg. window (scrc_refills cfg) (scrc_period cfg))
-                                       (sc_refill_cfgs_of s) (cur_sc s)"
+                                       (sc_refill_cfgs_of s) sc_ptr"
                in hoare_seq_ext)
    apply wpsimp
 
@@ -8944,42 +9105,44 @@ lemma handle_overrun_loop_head_bound:
 
   apply (intro hoare_vcg_conj_lift_pre_fix; (solves handle_overrun_loop_simple)?)
    defer
-   apply (wpsimp wp: schedule_used_window get_refills_wp set_refills_wp update_sched_context_wp
-               simp: refill_pop_head_def)
-   apply (clarsimp simp: vs_all_heap_simps obj_at_kh_kheap_simps pred_map_simps)
-   apply (rename_tac sc n)
-   apply (frule head_time_buffer_true_imp_unat_buffer[THEN iffD1, rotated])
-    apply (fastforce simp: vs_all_heap_simps obj_at_kh_kheap_simps)
-   apply (prop_tac "unat (r_time (refill_hd sc)) \<le> unat (r_time (hd (tl (sc_refills sc))))")
-    apply (subst hd_tl_nth)
-     apply (simp add: Suc_lessI)
-    apply (subst hd_conv_nth)
-     apply blast
-    apply (erule (1) ordered_disjoint_no_overflow_implies_sorted)
-      apply force
-     apply (simp add: Suc_lessI)
-    apply simp
+   apply (rule_tac f=cur_sc in hoare_lift_Pf2)
+    apply (wpsimp wp: schedule_used_window get_refills_wp set_refills_wp update_sched_context_wp
+                simp: refill_pop_head_def)
+    apply (clarsimp simp: vs_all_heap_simps obj_at_kh_kheap_simps pred_map_simps)
+    apply (rename_tac sc n)
+    apply (frule head_time_buffer_true_imp_unat_buffer[THEN iffD1, rotated])
+     apply (fastforce simp: vs_all_heap_simps obj_at_kh_kheap_simps)
+    apply (prop_tac "unat (r_time (refill_hd sc)) \<le> unat (r_time (hd (tl (sc_refills sc))))")
+     apply (subst hd_tl_nth)
+      apply (simp add: Suc_lessI)
+     apply (subst hd_conv_nth)
+      apply blast
+     apply (erule (1) ordered_disjoint_no_overflow_implies_sorted)
+       apply force
+      apply (simp add: Suc_lessI)
+     apply simp
 
-   apply (prop_tac "hd (tl (sc_refills sc)) \<in> set (sc_refills sc)")
-    apply (metis Nitpick.size_list_simp(2) hd_Cons_tl hd_in_set list.set_intros(2))
-   apply (frule (2) ordered_disjoint_last)
-   apply (intro conjI impI)
+    apply (prop_tac "hd (tl (sc_refills sc)) \<in> set (sc_refills sc)")
+     apply (metis Nitpick.size_list_simp(2) hd_Cons_tl hd_in_set list.set_intros(2))
+    apply (frule (2) ordered_disjoint_last)
+    apply (intro conjI impI)
+         apply (clarsimp simp: window_def)
+         apply (prop_tac "last (tl (sc_refills sc)) = refill_tl sc")
+          apply (metis Nitpick.size_list_simp(2) last_tl)
+         apply clarsimp
         apply (blast intro: ordered_disjoint_sublist)
-       apply (clarsimp simp: window_def)
-       apply (prop_tac "last (tl (sc_refills sc)) = refill_tl sc")
-        apply (metis Nitpick.size_list_simp(2) last_tl)
-       apply clarsimp
-      apply (blast intro: no_overflow_sublist)
-     apply (metis Nitpick.size_list_simp(2))
-    apply (rule word_add_le_mono1)
-     apply (clarsimp simp: word_le_nat_alt)
-    apply (frule (1) ordered_disjoint_last)
-     apply metis
-    apply (subst power_two_max_word_fold)
-    apply (clarsimp simp: unat_max_word word_le_nat_alt)
-    apply (rule le_imp_less_Suc)
-    apply (fastforce simp: window_def)
-   apply (fastforce simp: window_def word_le_nat_alt)
+       apply (blast intro: no_overflow_sublist)
+      apply (metis Nitpick.size_list_simp(2))
+     apply (rule word_add_le_mono1)
+      apply (clarsimp simp: word_le_nat_alt)
+     apply (frule (1) ordered_disjoint_last)
+      apply metis
+     apply (subst power_two_max_word_fold)
+     apply (clarsimp simp: unat_max_word word_le_nat_alt)
+     apply (rule le_imp_less_Suc)
+     apply (fastforce simp: window_def)
+    apply (fastforce simp: window_def word_le_nat_alt)
+   apply wpsimp
 
   apply (wpsimp wp: get_refills_wp set_refills_wp update_sched_context_wp
               simp: refill_pop_head_def schedule_used_defs)
@@ -9012,11 +9175,14 @@ lemma handle_overrun_loop_head_bound:
             not_less_eq_eq numerals(2) order_refl)
 
 lemma schedule_used_refills_sum:
-  "\<lbrace>\<lambda>s. pred_map (\<lambda>cfg. refills_sum (scrc_refills cfg) + r_amount new = scrc_budget cfg)
-                 (sc_refill_cfgs_of s) (cur_sc s) \<and> sc_ptr = cur_sc s\<rbrace>
-   schedule_used sc_ptr new
+  "\<lbrace>\<lambda>s. if sc_ptr' = sc_ptr
+        then pred_map (\<lambda>cfg. refills_sum (scrc_refills cfg) + r_amount new = scrc_budget cfg)
+                      (sc_refill_cfgs_of s) sc_ptr
+        else pred_map (\<lambda>cfg. refills_sum (scrc_refills cfg) = (scrc_budget cfg))
+                   (sc_refill_cfgs_of s) sc_ptr\<rbrace>
+   schedule_used sc_ptr' new
    \<lbrace>\<lambda>_ s. pred_map (\<lambda>cfg. refills_sum (scrc_refills cfg) = (scrc_budget cfg))
-                   (sc_refill_cfgs_of s) (cur_sc s)\<rbrace>"
+                   (sc_refill_cfgs_of s) sc_ptr\<rbrace>"
   apply (wpsimp wp: update_sched_context_wp get_refills_wp
               simp: schedule_used_defs refill_add_tail_def update_refill_tl_def)
   apply (rename_tac sc n)
@@ -9039,10 +9205,12 @@ lemma schedule_used_refills_sum:
   done
 
 lemma handle_overrun_loop_body_refills_sum:
-  "\<lbrace>\<lambda>s. pred_map (\<lambda>cfg. refills_sum (scrc_refills cfg) = scrc_budget cfg) (sc_refill_cfgs_of s) (cur_sc s)
-        \<and> pred_map (\<lambda>cfg. scrc_refills cfg \<noteq> []) (sc_refill_cfgs_of s) (cur_sc s)\<rbrace>
+  "\<lbrace>\<lambda>s. pred_map (\<lambda>cfg. refills_sum (scrc_refills cfg) = scrc_budget cfg)
+                      (sc_refill_cfgs_of s) sc_ptr
+        \<and> (sc_ptr = cur_sc s \<longrightarrow> pred_map (\<lambda>cfg. scrc_refills cfg \<noteq> []) (sc_refill_cfgs_of s) sc_ptr)\<rbrace>
    handle_overrun_loop_body r
-   \<lbrace>\<lambda>_ s. pred_map (\<lambda>cfg. refills_sum (scrc_refills cfg) = scrc_budget cfg) (sc_refill_cfgs_of s) (cur_sc s)\<rbrace>"
+   \<lbrace>\<lambda>_ s. pred_map (\<lambda>cfg. refills_sum (scrc_refills cfg) = scrc_budget cfg)
+                    (sc_refill_cfgs_of s) sc_ptr\<rbrace>"
   (is "valid _ _ (\<lambda>_ s. ?post s)")
   apply (clarsimp simp: handle_overrun_loop_body_def)
   apply (rule hoare_seq_ext[OF _ gets_sp])
@@ -9063,50 +9231,38 @@ lemma handle_overrun_loop_body_refills_sum:
   done
 
 lemma handle_overrun_loop_refills_sum:
-  "\<lbrace>\<lambda>s. pred_map (\<lambda>cfg. refills_sum (scrc_refills cfg) = scrc_budget cfg) (sc_refill_cfgs_of s) (cur_sc s)
-        \<and> pred_map (\<lambda>cfg. scrc_refills cfg \<noteq> []) (sc_refill_cfgs_of s) (cur_sc s)
-        \<and> sc_ptr = cur_sc s\<rbrace>
+  "\<lbrace>\<lambda>s. pred_map (\<lambda>cfg. refills_sum (scrc_refills cfg) = scrc_budget cfg)
+                      (sc_refill_cfgs_of s) sc_ptr
+        \<and> (sc_ptr = cur_sc s \<longrightarrow> pred_map (\<lambda>cfg. scrc_refills cfg \<noteq> []) (sc_refill_cfgs_of s) sc_ptr)\<rbrace>
    handle_overrun_loop usage
-   \<lbrace>\<lambda>_ s. pred_map (\<lambda>cfg. refills_sum (scrc_refills cfg) = scrc_budget cfg) (sc_refill_cfgs_of s) (cur_sc s)\<rbrace>"
+   \<lbrace>\<lambda>_ s. pred_map (\<lambda>cfg. refills_sum (scrc_refills cfg) = scrc_budget cfg)
+                    (sc_refill_cfgs_of s) sc_ptr\<rbrace>"
   (is "valid ?pre _ _")
+  supply if_split[split del]
   apply (clarsimp simp: handle_overrun_loop_def)
   apply (wpsimp wp: valid_whileLoop[where I="\<lambda>_. ?pre"]
          ; fastforce?)
-  apply (wpsimp wp: handle_overrun_loop_body_refills_sum handle_overrun_loop_body_nonzero_refills)
+  apply (intro hoare_vcg_conj_lift_pre_fix; (solves handle_overrun_loop_body_simple)?)
+  apply (wpsimp wp: handle_overrun_loop_body_refills_sum)
   done
 
-method head_insufficient_loop_simple
-  = ((clarsimp simp: head_insufficient_loop_def)?
-     , wpsimp wp: whileLoop_wp' set_refills_wp get_refills_wp
-            simp: non_overlapping_merge_refills_def refill_pop_head_def schedule_used_defs
-                  update_sched_context_set_refills_rewrite update_refill_hd_rewrite
-     , clarsimp simp: vs_all_heap_simps obj_at_def sc_valid_refills_def round_robin_def
-                      unat_MAX_RELEASE_TIME
-               split: if_splits
-     , fastforce?)
-
-method refill_head_overlapping_loop_simple
-  = ((clarsimp simp: refill_head_overlapping_loop_def)?
-     , wpsimp wp: whileLoop_wp' set_refills_wp get_refills_wp
-            simp: merge_refills_def round_robin_def refill_pop_head_def sc_valid_refills_def
-                  update_sched_context_set_refills_rewrite update_refill_hd_rewrite
-                  vs_all_heap_simps obj_at_def)
-
 lemma head_insufficient_loop_round_robin[wp]:
-  "head_insufficient_loop sc_ptr \<lbrace>\<lambda>s. P (round_robin (cur_sc s) s)\<rbrace>"
+  "head_insufficient_loop sc_ptr' \<lbrace>\<lambda>s. P (round_robin sc_ptr s)\<rbrace>"
   apply head_insufficient_loop_simple
   done
 
 lemma handle_overrun_loop_round_robin[wp]:
-  "handle_overrun_loop sc_ptr \<lbrace>\<lambda>s. P (round_robin (cur_sc s) s)\<rbrace>"
+  "handle_overrun_loop sc_ptr' \<lbrace>\<lambda>s. P (round_robin sc_ptr s)\<rbrace>"
   apply handle_overrun_loop_simple
   done
 
 lemma handle_overrun_loop_body_length:
-  "\<lbrace>\<lambda>s. pred_map (\<lambda>cfg. length (scrc_refills cfg) \<le> scrc_refill_max cfg) (sc_refill_cfgs_of s) (cur_sc s)
-        \<and> pred_map (\<lambda>cfg. scrc_refills cfg \<noteq> []) (sc_refill_cfgs_of s) (cur_sc s) \<rbrace>
+  "\<lbrace>\<lambda>s. pred_map (\<lambda>cfg. length (scrc_refills cfg) \<le> scrc_refill_max cfg)
+                      (sc_refill_cfgs_of s) sc_ptr
+        \<and> (sc_ptr = cur_sc s \<longrightarrow> pred_map (\<lambda>cfg. scrc_refills cfg \<noteq> []) (sc_refill_cfgs_of s) sc_ptr)\<rbrace>
    handle_overrun_loop_body usage
-   \<lbrace>\<lambda>_ s. pred_map (\<lambda>cfg. length (scrc_refills cfg) \<le> scrc_refill_max cfg) (sc_refill_cfgs_of s) (cur_sc s)\<rbrace>"
+   \<lbrace>\<lambda>_ s. pred_map (\<lambda>cfg. length (scrc_refills cfg) \<le> scrc_refill_max cfg)
+                    (sc_refill_cfgs_of s) sc_ptr\<rbrace>"
   (is "valid _ _ (\<lambda>_ s. ?post s)")
   apply handle_overrun_loop_body_simple
   apply (rename_tac sc n)
@@ -9114,16 +9270,18 @@ lemma handle_overrun_loop_body_length:
   done
 
 lemma handle_overrun_loop_length:
-  "\<lbrace>\<lambda>s. pred_map (\<lambda>cfg. length (scrc_refills cfg) \<le> scrc_refill_max cfg) (sc_refill_cfgs_of s) (cur_sc s)
-        \<and> pred_map (\<lambda>cfg. scrc_refills cfg \<noteq> []) (sc_refill_cfgs_of s) (cur_sc s)\<rbrace>
+  "\<lbrace>\<lambda>s. pred_map (\<lambda>cfg. length (scrc_refills cfg) \<le> scrc_refill_max cfg)
+                      (sc_refill_cfgs_of s) sc_ptr
+        \<and> (sc_ptr = cur_sc s \<longrightarrow> pred_map (\<lambda>cfg. scrc_refills cfg \<noteq> []) (sc_refill_cfgs_of s) sc_ptr)\<rbrace>
    handle_overrun_loop usage
-   \<lbrace>\<lambda>_ s. pred_map (\<lambda>cfg. length (scrc_refills cfg) \<le> scrc_refill_max cfg) (sc_refill_cfgs_of s) (cur_sc s)\<rbrace>"
+   \<lbrace>\<lambda>_ s. pred_map (\<lambda>cfg. length (scrc_refills cfg) \<le> scrc_refill_max cfg)
+                    (sc_refill_cfgs_of s) sc_ptr\<rbrace>"
   (is "valid ?pre _ _")
+  supply if_split[split del]
   apply (clarsimp simp: handle_overrun_loop_def)
-  apply (rule_tac I="\<lambda>_. ?pre" in valid_whileLoop)
-    apply (wpsimp wp: whileLoop_wp' handle_overrun_loop_body_nonzero_refills
-                      handle_overrun_loop_body_length
-           | wps)+
+  apply (rule_tac I="\<lambda>_. ?pre" in valid_whileLoop; (solves simp)?)
+  apply (intro hoare_vcg_conj_lift_pre_fix; (solves handle_overrun_loop_body_simple)?)
+  apply (wpsimp wp: handle_overrun_loop_body_length)
   done
 
 lemma handle_overrun_loop_body_scs_of_cur_sc[wp]:
@@ -9175,37 +9333,37 @@ lemma refill_budget_check_no_overflow_helper:
   done
 
 lemma refill_budget_check_refills_sum_helper:
-  "\<lbrace>\<lambda>s. all_sp_valid_refills_but_MIN_BUDGET_in_head_no_overflow (cur_sc s) s
+  "\<lbrace>\<lambda>s. all_sp_valid_refills_but_MIN_BUDGET_in_head_no_overflow sc_ptr s
         \<and> pred_map (\<lambda>cfg. refills_unat_sum (scrc_refills cfg) = unat (scrc_budget cfg))
-                    (sc_refill_cfgs_of s) (cur_sc s)
-        \<and> cur_sc s = csc_ptr\<rbrace>
+                    (sc_refill_cfgs_of s) sc_ptr\<rbrace>
    do y \<leftarrow> update_refill_hd csc_ptr (r_time_update (\<lambda>t. t + u) \<circ> r_amount_update (\<lambda>m. m - u));
-           schedule_used csc_ptr \<lparr>r_time = r_time (refill_hd sc) + sc_period sc, r_amount = u\<rparr>
+      schedule_used csc_ptr \<lparr>r_time = r_time (refill_hd sc) + sc_period sc, r_amount = u\<rparr>
    od
    \<lbrace>\<lambda>_ s. pred_map (\<lambda>cfg. refills_sum (scrc_refills cfg) = scrc_budget cfg)
-                    (sc_refill_cfgs_of s) (cur_sc s)\<rbrace>"
-  apply (wpsimp wp: schedule_used_refills_sum set_refills_wp get_refills_wp
-              simp: update_refill_hd_rewrite)
-  apply (clarsimp simp: obj_at_def vs_all_heap_simps)
-  apply (case_tac "sc_refills sc"; simp)
+                    (sc_refill_cfgs_of s) sc_ptr\<rbrace>"
+  apply (rule_tac f=cur_sc in hoare_lift_Pf2)
+   apply (wpsimp wp: schedule_used_refills_sum set_refills_wp get_refills_wp
+               simp: update_refill_hd_rewrite)
+   apply (clarsimp simp: obj_at_def vs_all_heap_simps)
+   apply (case_tac "sc_refills sc"; simp)
+  apply wpsimp
   done
 
 lemma refill_budget_check_ordered_disjoint_helper':
   "r_time (hd refills) < MAX_RELEASE_TIME \<Longrightarrow>
-   \<lbrace>\<lambda>s. all_sp_valid_refills_but_MIN_BUDGET_in_head (cur_sc s) s
+   \<lbrace>\<lambda>s. all_sp_valid_refills_but_MIN_BUDGET_in_head sc_ptr s
         \<and> pred_map (\<lambda>cfg. unat (r_time (scrc_refill_hd cfg)) + 4 * unat MAX_PERIOD
                            \<le> unat max_time)
-                    (sc_refill_cfgs_of s) (cur_sc s)
-        \<and> cur_sc s = csc_ptr
+                    (sc_refill_cfgs_of s) sc_ptr
         \<and> (pred_map (\<lambda>cfg. r_time (scrc_refill_hd cfg) < MAX_RELEASE_TIME)
-                     (sc_refill_cfgs_of s) (cur_sc s)
-            \<longrightarrow> pred_map (\<lambda>cfg. u < r_amount (scrc_refill_hd cfg)) (sc_refill_cfgs_of s) (cur_sc s))
-        \<and> (\<exists>sc n. ko_at (SchedContext sc n) csc_ptr s \<and> refills = sc_refills sc)
-        \<and> (\<exists>n. ko_at (SchedContext sc n) csc_ptr s)\<rbrace>
+                     (sc_refill_cfgs_of s) sc_ptr
+            \<longrightarrow> pred_map (\<lambda>cfg. u < r_amount (scrc_refill_hd cfg)) (sc_refill_cfgs_of s) sc_ptr)
+        \<and> (\<exists>sc n. ko_at (SchedContext sc n) sc_ptr s \<and> refills = sc_refills sc)
+        \<and> (\<exists>n. ko_at (SchedContext sc n) sc_ptr s)\<rbrace>
    do y \<leftarrow> update_refill_hd csc_ptr (r_time_update (\<lambda>t. t + u) \<circ> r_amount_update (\<lambda>m. m - u));
-           schedule_used csc_ptr \<lparr>r_time = r_time (refill_hd sc) + sc_period sc, r_amount = u\<rparr>
+      schedule_used csc_ptr \<lparr>r_time = r_time (refill_hd sc) + sc_period sc, r_amount = u\<rparr>
    od
-   \<lbrace>\<lambda>_ s. pred_map (\<lambda>cfg. ordered_disjoint (scrc_refills cfg)) (sc_refill_cfgs_of s) (cur_sc s)\<rbrace>"
+   \<lbrace>\<lambda>_ s. pred_map (\<lambda>cfg. ordered_disjoint (scrc_refills cfg)) (sc_refill_cfgs_of s) sc_ptr\<rbrace>"
   apply (wpsimp wp: schedule_used_ordered_disjoint set_refills_wp get_refills_wp
               simp: update_refill_hd_rewrite)
   apply (clarsimp simp: obj_at_def vs_all_heap_simps)
@@ -9235,22 +9393,21 @@ lemma refill_budget_check_ordered_disjoint_helper':
 
 lemma refill_budget_check_no_overflow':
   "r_time (hd refills) < MAX_RELEASE_TIME \<Longrightarrow>
-   \<lbrace>\<lambda>s. all_sp_valid_refills_but_MIN_BUDGET_in_head (cur_sc s) s
+   \<lbrace>\<lambda>s. all_sp_valid_refills_but_MIN_BUDGET_in_head sc_ptr s
         \<and> pred_map (\<lambda>cfg. refills_unat_sum (scrc_refills cfg) = unat (scrc_budget cfg))
-                    (sc_refill_cfgs_of s) (cur_sc s)
+                    (sc_refill_cfgs_of s) sc_ptr
         \<and> pred_map (\<lambda>cfg. unat (r_time (scrc_refill_hd cfg)) + 4 * unat MAX_PERIOD
                            \<le> unat max_time)
-                    (sc_refill_cfgs_of s) (cur_sc s)
-        \<and> cur_sc s = csc_ptr
+                    (sc_refill_cfgs_of s) sc_ptr
         \<and> (pred_map (\<lambda>cfg. r_time (scrc_refill_hd cfg) < MAX_RELEASE_TIME)
-                     (sc_refill_cfgs_of s) (cur_sc s)
-            \<longrightarrow> pred_map (\<lambda>cfg. u < r_amount (scrc_refill_hd cfg)) (sc_refill_cfgs_of s) (cur_sc s))
-        \<and> (\<exists>sc n. ko_at (SchedContext sc n) csc_ptr s \<and> refills = sc_refills sc)
-        \<and> (\<exists>n. ko_at (SchedContext sc n) csc_ptr s)\<rbrace>
+                     (sc_refill_cfgs_of s) sc_ptr
+            \<longrightarrow> pred_map (\<lambda>cfg. u < r_amount (scrc_refill_hd cfg)) (sc_refill_cfgs_of s) sc_ptr)
+        \<and> (\<exists>sc n. ko_at (SchedContext sc n) sc_ptr s \<and> refills = sc_refills sc)
+        \<and> (\<exists>n. ko_at (SchedContext sc n) sc_ptr s)\<rbrace>
    do y \<leftarrow> update_refill_hd csc_ptr (r_time_update (\<lambda>t. t + u) \<circ> r_amount_update (\<lambda>m. m - u));
-           schedule_used csc_ptr \<lparr>r_time = r_time (refill_hd sc) + sc_period sc, r_amount = u\<rparr>
+      schedule_used csc_ptr \<lparr>r_time = r_time (refill_hd sc) + sc_period sc, r_amount = u\<rparr>
    od
-   \<lbrace>\<lambda>_ s. pred_map (\<lambda>cfg. no_overflow (scrc_refills cfg)) (sc_refill_cfgs_of s) (cur_sc s)\<rbrace>"
+   \<lbrace>\<lambda>_ s. pred_map (\<lambda>cfg. no_overflow (scrc_refills cfg)) (sc_refill_cfgs_of s) sc_ptr\<rbrace>"
   apply (wpsimp wp: schedule_used_no_overflow set_refills_wp get_refills_wp
               simp: update_refill_hd_rewrite)
   apply (clarsimp simp: obj_at_def vs_all_heap_simps)
@@ -9293,42 +9450,40 @@ lemma refill_budget_check_no_overflow':
 
 lemma refill_budget_check_window_helper:
   "r_time (hd refills) < MAX_RELEASE_TIME \<Longrightarrow>
-   \<lbrace>\<lambda>s. all_sp_valid_refills_but_MIN_BUDGET_in_head (cur_sc s) s
+   \<lbrace>\<lambda>s. all_sp_valid_refills_but_MIN_BUDGET_in_head sc_ptr s
         \<and> pred_map (\<lambda>cfg. unat (r_time (scrc_refill_hd cfg)) + 4 * unat MAX_PERIOD
                            \<le> unat max_time)
-                    (sc_refill_cfgs_of s) (cur_sc s)
-        \<and> cur_sc s = csc_ptr
+                    (sc_refill_cfgs_of s) sc_ptr
         \<and> (pred_map (\<lambda>cfg. r_time (scrc_refill_hd cfg) < MAX_RELEASE_TIME)
-                     (sc_refill_cfgs_of s) (cur_sc s)
-           \<longrightarrow> pred_map (\<lambda>cfg. u < r_amount (scrc_refill_hd cfg)) (sc_refill_cfgs_of s) (cur_sc s))
-        \<and> (\<exists>sc n. ko_at (SchedContext sc n) csc_ptr s \<and> refills = sc_refills sc)
-        \<and> (\<exists>n. ko_at (SchedContext sc n) csc_ptr s)\<rbrace>
+                     (sc_refill_cfgs_of s) sc_ptr
+           \<longrightarrow> pred_map (\<lambda>cfg. u < r_amount (scrc_refill_hd cfg)) (sc_refill_cfgs_of s) sc_ptr)
+        \<and> (\<exists>sc n. ko_at (SchedContext sc n) sc_ptr s \<and> refills = sc_refills sc)
+        \<and> (\<exists>n. ko_at (SchedContext sc n) sc_ptr s)\<rbrace>
    do y \<leftarrow> update_refill_hd csc_ptr (r_time_update (\<lambda>t. t + u) \<circ> r_amount_update (\<lambda>m. m - u));
-           schedule_used csc_ptr \<lparr>r_time = r_time (refill_hd sc) + sc_period sc, r_amount = u\<rparr>
+      schedule_used csc_ptr \<lparr>r_time = r_time (refill_hd sc) + sc_period sc, r_amount = u\<rparr>
    od
-   \<lbrace>\<lambda>_ s. pred_map (\<lambda>cfg. window (scrc_refills cfg) (scrc_period cfg)) (sc_refill_cfgs_of s) (cur_sc s)\<rbrace>"
+   \<lbrace>\<lambda>_ s. pred_map (\<lambda>cfg. window (scrc_refills cfg) (scrc_period cfg)) (sc_refill_cfgs_of s) sc_ptr\<rbrace>"
   apply (wpsimp wp: schedule_used_window set_refills_wp get_refills_wp
               simp: update_refill_hd_rewrite)
   apply (clarsimp simp: obj_at_def vs_all_heap_simps)
   apply (frule_tac refill="refill_hd sc" in refill_budget_check_refill_amount_helper; simp?)
   apply (intro conjI impI allI)
-      apply (fastforce intro: refill_budget_check_ordered_disjoint_helper)
-     apply (fastforce simp: unat_add_lem'' word_less_nat_alt word_le_nat_alt window_def last_tl)
+      apply (fastforce simp: unat_add_lem'' word_less_nat_alt word_le_nat_alt window_def last_tl)
+     apply (fastforce intro: refill_budget_check_ordered_disjoint_helper)
     apply (fastforce intro: refill_budget_check_no_overflow_helper)
    apply (fastforce simp: unat_add_lem'' word_less_nat_alt word_le_nat_alt)
   apply (fastforce simp: unat_add_lem'' word_less_nat_alt word_le_nat_alt)
   done
 
 lemma refill_budget_check_length_helper:
-  "\<lbrace>\<lambda>s. pred_map (\<lambda>cfg. 0 < length (scrc_refills cfg)) (sc_refill_cfgs_of s) (cur_sc s)
+  "\<lbrace>\<lambda>s. pred_map (\<lambda>cfg. 0 < length (scrc_refills cfg)) (sc_refill_cfgs_of s) sc_ptr
         \<and> pred_map (\<lambda>cfg. length (scrc_refills cfg) \<le> scrc_refill_max cfg)
-                    (sc_refill_cfgs_of s) (cur_sc s)
-        \<and> cur_sc s = csc_ptr\<rbrace>
+                    (sc_refill_cfgs_of s) sc_ptr \<and> sc_ptr = csc_ptr\<rbrace>
    do y \<leftarrow> update_refill_hd csc_ptr (r_time_update (\<lambda>t. t + u) \<circ> r_amount_update (\<lambda>m. m - u));
-           schedule_used csc_ptr \<lparr>r_time = r_time (refill_hd sc) + sc_period sc, r_amount = u\<rparr>
+      schedule_used csc_ptr \<lparr>r_time = r_time (refill_hd sc) + sc_period sc, r_amount = u\<rparr>
    od
    \<lbrace>\<lambda>_ s. pred_map (\<lambda>cfg. length (scrc_refills cfg) \<le> scrc_refill_max cfg)
-                   (sc_refill_cfgs_of s) (cur_sc s)\<rbrace>"
+                   (sc_refill_cfgs_of s) sc_ptr\<rbrace>"
   apply (wpsimp wp: set_refills_wp get_refills_wp
               simp: vs_all_heap_simps update_sched_context_set_refills_rewrite
                     update_refill_hd_rewrite schedule_used_defs)
@@ -9339,24 +9494,196 @@ lemma refill_budget_check_length_helper:
 
 lemma refill_budget_check_refills_unat_sum_helper:
   "r_time (hd refills) < MAX_RELEASE_TIME \<Longrightarrow>
-   \<lbrace>\<lambda>s. all_sp_valid_refills_but_MIN_BUDGET_in_head_no_overflow (cur_sc s) s
+   \<lbrace>\<lambda>s. all_sp_valid_refills_but_MIN_BUDGET_in_head_no_overflow sc_ptr s
         \<and> pred_map (\<lambda>cfg. refills_unat_sum (scrc_refills cfg) = unat (scrc_budget cfg))
-                    (sc_refill_cfgs_of s) (cur_sc s)
-        \<and> cur_sc s = csc_ptr
+                    (sc_refill_cfgs_of s) sc_ptr
         \<and> (pred_map (\<lambda>cfg. r_time (scrc_refill_hd cfg) < MAX_RELEASE_TIME)
-                     (sc_refill_cfgs_of s) (cur_sc s)
-           \<longrightarrow> pred_map (\<lambda>cfg. u < r_amount (scrc_refill_hd cfg)) (sc_refill_cfgs_of s) (cur_sc s))
-        \<and> (\<exists>sc n. ko_at (SchedContext sc n) csc_ptr s \<and> refills = sc_refills sc)\<rbrace>
-   do y <- update_refill_hd csc_ptr (r_time_update (\<lambda>t. t + u) \<circ> r_amount_update (\<lambda>m. m - u));
-           schedule_used csc_ptr \<lparr>r_time = r_time (refill_hd sc) + sc_period sc, r_amount = u\<rparr>
+                     (sc_refill_cfgs_of s) sc_ptr
+           \<longrightarrow> pred_map (\<lambda>cfg. u < r_amount (scrc_refill_hd cfg)) (sc_refill_cfgs_of s) sc_ptr)
+        \<and> (\<exists>sc n. ko_at (SchedContext sc n) sc_ptr s \<and> refills = sc_refills sc)\<rbrace>
+   do y \<leftarrow> update_refill_hd csc_ptr (r_time_update (\<lambda>t. t + u) \<circ> r_amount_update (\<lambda>m. m - u));
+      schedule_used csc_ptr \<lparr>r_time = r_time (refill_hd sc) + sc_period sc, r_amount = u\<rparr>
    od
    \<lbrace>\<lambda>_ s. pred_map (\<lambda>cfg. refills_unat_sum (scrc_refills cfg) = unat (scrc_budget cfg))
-                   (sc_refill_cfgs_of s) (cur_sc s)\<rbrace>"
+                   (sc_refill_cfgs_of s) sc_ptr\<rbrace>"
   apply (wpsimp wp: schedule_used_refills_unat_sum set_refills_wp get_refills_wp
               simp: update_refill_hd_rewrite)
   apply (clarsimp simp: obj_at_def vs_all_heap_simps)
   apply (fastforce dest: refill_budget_check_refills_unat_sum_word_helper
                    simp: refills_unat_sum_def)
+  done
+
+lemma schedule_used_non_zero_refills:
+  "\<lbrace>\<lambda>s. pred_map (\<lambda>cfg. \<forall>refill \<in> set (scrc_refills cfg). 0 < unat (r_amount refill))
+                      (sc_refill_cfgs_of s) sc_ptr
+        \<and> (sc_ptr' = sc_ptr
+           \<longrightarrow> pred_map (\<lambda>cfg. refills_unat_sum ((scrc_refills cfg) @ [new]) \<le> unat (scrc_budget cfg))
+                        (sc_refill_cfgs_of s) sc_ptr
+               \<and> 0 < unat (r_amount new))\<rbrace>
+   schedule_used sc_ptr' new
+   \<lbrace>\<lambda>_ s. pred_map (\<lambda>cfg. \<forall>refill \<in> set (scrc_refills cfg). 0 < unat (r_amount refill))
+            (sc_refill_cfgs_of s) sc_ptr\<rbrace>"
+  supply map_map[simp del]
+  apply schedule_used_simple
+  apply (prop_tac " 0 < unat (r_amount (refill_tl sc) + r_amount new)")
+   apply (subst unat_add_lem'')
+    apply (clarsimp simp: refills_unat_sum_append)
+    apply (prop_tac "unat (r_amount (refill_tl sc)) \<le> refills_unat_sum (sc_refills sc)")
+     apply (fastforce intro: refills_unat_sum_member_bound last_in_set)
+    apply (rule_tac y="unat (sc_budget sc)" in order_trans)
+     apply linarith
+    apply simp
+   apply blast
+  apply (meson in_set_butlastD)
+  done
+
+crunches refill_pop_head
+   for non_zero_refills[wp]:
+         "\<lambda>s. pred_map (\<lambda>cfg. \<forall>refill \<in> set (scrc_refills cfg). 0 < unat (r_amount refill))
+                       (sc_refill_cfgs_of s) sc_ptr"
+   (wp: crunch_wps update_sched_context_wp)
+
+lemma handle_overrun_loop_body_non_zero_refills:
+  "\<lbrace>\<lambda>s. if sc_ptr = cur_sc s
+        then pred_map (\<lambda>cfg. \<forall>refill \<in> set (scrc_refills cfg). 0 < unat (r_amount refill))
+                      (sc_refill_cfgs_of s) sc_ptr
+             \<and> pred_map (\<lambda>cfg. scrc_refills cfg \<noteq> []) (sc_refill_cfgs_of s) sc_ptr
+             \<and> pred_map (\<lambda>cfg. refills_unat_sum (scrc_refills cfg) = unat (scrc_budget cfg))
+                        (sc_refill_cfgs_of s) sc_ptr
+        else pred_map (\<lambda>cfg. \<forall>refill \<in> set (scrc_refills cfg). 0 < unat (r_amount refill))
+                   (sc_refill_cfgs_of s) sc_ptr\<rbrace>
+   handle_overrun_loop_body usage
+   \<lbrace>\<lambda>_ s. pred_map (\<lambda>cfg. \<forall>refill \<in> set (scrc_refills cfg). 0 < unat (r_amount refill))
+                   (sc_refill_cfgs_of s) sc_ptr\<rbrace>"
+  (is "\<lbrace>_\<rbrace> _ \<lbrace>\<lambda>_. ?Q\<rbrace>")
+  supply map_map[simp del] list.set_sel[simp add]
+  apply (clarsimp simp: handle_overrun_loop_body_def)
+  apply (rule hoare_seq_ext[OF _ gets_sp], rename_tac csc_ptr)
+  apply (rule hoare_seq_ext_skip, wpsimp simp: refill_single_def refill_size_def)
+  apply (rule hoare_seq_ext_skip, wpsimp)
+  apply (rule_tac B="\<lambda>_ s. ?Q s \<and> csc_ptr = cur_sc s" in hoare_seq_ext)
+   apply wpsimp
+  apply (rule hoare_if)
+   apply (wpsimp wp: update_sched_context_wp
+               simp: update_refill_hd_def)
+   apply (clarsimp simp: vs_all_heap_simps obj_at_def)
+  apply (intro hoare_vcg_conj_lift_pre_fix; (solves wpsimp)?)
+  apply (wpsimp wp: schedule_used_non_zero_refills update_sched_context_wp get_refills_wp
+              simp: refill_pop_head_def)
+  apply (clarsimp simp: vs_all_heap_simps obj_at_def refills_unat_sum_def)
+  apply (intro conjI impI; force?)
+  apply (clarsimp simp: vs_all_heap_simps obj_at_def refills_unat_sum_def)
+  apply (rename_tac sc n)
+  apply (case_tac "sc_refills sc"; clarsimp)
+  done
+
+lemma handle_overrun_loop_non_zero_refills:
+  "\<lbrace>\<lambda>s. pred_map (\<lambda>cfg. \<forall>refill \<in> set (scrc_refills cfg). 0 < unat (r_amount refill))
+                      (sc_refill_cfgs_of s) sc_ptr
+        \<and> (sc_ptr = cur_sc s
+           \<longrightarrow>  pred_map (\<lambda>cfg. scrc_refills cfg \<noteq> []) (sc_refill_cfgs_of s) sc_ptr
+                \<and> pred_map (\<lambda>cfg. refills_unat_sum (scrc_refills cfg) = unat (scrc_budget cfg))
+                           (sc_refill_cfgs_of s) sc_ptr)\<rbrace>
+   handle_overrun_loop usage
+   \<lbrace>\<lambda>_ s. pred_map (\<lambda>cfg. \<forall>refill\<in>set (scrc_refills cfg). 0 < unat (r_amount refill))
+                   (sc_refill_cfgs_of s) sc_ptr\<rbrace>"
+  (is "valid ?pre _ _")
+  supply if_split[split del]
+  apply (clarsimp simp: handle_overrun_loop_def)
+  apply (rule_tac I="\<lambda>_. ?pre" in valid_whileLoop; (solves simp)?)
+  apply (intro hoare_vcg_conj_lift_pre_fix; (solves handle_overrun_loop_body_simple)?)
+   apply (wpsimp wp: handle_overrun_loop_body_non_zero_refills)
+   apply (clarsimp split: if_splits)
+  apply (rule hoare_imp_helper; (solves simp)?)
+   apply (wpsimp wp: handle_overrun_loop_body_refills_unat_sum_equals_budget)
+  apply (wpsimp wp: handle_overrun_loop_body_non_zero_refills)
+  done
+
+lemma non_overlapping_merge_refills_non_zero_refills:
+  "\<lbrace>\<lambda>s. pred_map (\<lambda>cfg. \<forall>refill\<in>set (scrc_refills cfg). 0 < unat (r_amount refill))
+                      (sc_refill_cfgs_of s) sc_ptr
+        \<and> (sc_ptr' = sc_ptr
+           \<longrightarrow> pred_map (\<lambda>cfg. scrc_refills cfg \<noteq> []) (sc_refill_cfgs_of s) sc_ptr
+               \<and> pred_map (\<lambda>cfg. unat MIN_BUDGET \<le> refills_unat_sum (scrc_refills cfg))
+                          (sc_refill_cfgs_of s) sc_ptr
+               \<and> pred_map (\<lambda>cfg. refills_unat_sum (scrc_refills cfg) = unat (scrc_budget cfg))
+                          (sc_refill_cfgs_of s) sc_ptr
+               \<and> the (head_insufficient sc_ptr s))\<rbrace>
+   non_overlapping_merge_refills sc_ptr'
+   \<lbrace>\<lambda>_ s. pred_map (\<lambda>cfg. \<forall>refill\<in>set (scrc_refills cfg). 0 < unat (r_amount refill))
+                   (sc_refill_cfgs_of s) sc_ptr\<rbrace>"
+  apply non_overlapping_merge_refills_simple
+  apply (frule head_insufficient_length_at_least_two[rotated])
+   apply (clarsimp simp: vs_all_heap_simps)
+  apply (intro conjI impI)
+   apply (subst unat_add_lem'')
+    apply (case_tac "sc_refills sc"; clarsimp)
+    apply (clarsimp simp: refills_unat_sum_cons)
+    apply (rule_tac y="unat (sc_budget sc)" in order_trans)
+     apply (prop_tac "unat (r_amount (hd list)) \<le> refills_unat_sum list")
+      apply (prop_tac "hd list \<in> set list")
+       apply (clarsimp simp: vs_all_heap_simps)
+      apply (frule_tac refill="hd list" in refills_unat_sum_member_bound[rotated])
+       apply (fastforce dest: refills_unat_sum_member_bound simp: vs_all_heap_simps)
+      apply fast
+     apply linarith
+    apply fastforce
+   apply simp
+  apply (metis list.sel(2) list.set_sel(2))
+  done
+
+lemma head_insufficient_loop_non_zero_refills:
+  "\<lbrace>\<lambda>s. pred_map (\<lambda>cfg. \<forall>refill \<in> set (scrc_refills cfg). 0 < unat (r_amount refill))
+                      (sc_refill_cfgs_of s) sc_ptr
+        \<and> (sc_ptr' = sc_ptr
+           \<longrightarrow> pred_map (\<lambda>cfg. scrc_refills cfg \<noteq> []) (sc_refill_cfgs_of s) sc_ptr
+               \<and> pred_map (\<lambda>cfg. unat MIN_BUDGET \<le> refills_unat_sum (scrc_refills cfg))
+                          (sc_refill_cfgs_of s) sc_ptr
+               \<and> pred_map (\<lambda>cfg. refills_unat_sum (scrc_refills cfg) = unat (scrc_budget cfg))
+                          (sc_refill_cfgs_of s) sc_ptr)\<rbrace>
+   head_insufficient_loop sc_ptr'
+   \<lbrace>\<lambda>_ s. pred_map (\<lambda>cfg. \<forall>refill \<in> set (scrc_refills cfg). 0 < unat (r_amount refill))
+                   (sc_refill_cfgs_of s) sc_ptr\<rbrace>"
+  (is "\<lbrace>?P\<rbrace> _ \<lbrace>_\<rbrace>")
+  apply (clarsimp simp: head_insufficient_loop_def)
+  apply (rule_tac I="\<lambda>_. ?P" in valid_whileLoop; fastforce?)
+  apply (intro hoare_vcg_conj_lift_pre_fix; (solves non_overlapping_merge_refills_simple)?)
+   apply (wpsimp wp: non_overlapping_merge_refills_non_zero_refills)
+  apply (rule hoare_imp_helper)
+   apply (intro hoare_vcg_conj_lift_pre_fix; (solves non_overlapping_merge_refills_simple)?)
+    apply (wpsimp wp: non_overlapping_merge_refills_refills_unat_sum_lower_bound)
+    apply (fastforce dest!: head_insufficient_length_at_least_two[rotated]
+                      simp: vs_all_heap_simps)
+   apply (wpsimp wp: non_overlapping_merge_refills_refills_unat_sum_equals_budget)
+   apply (fastforce dest!: head_insufficient_length_at_least_two[rotated]
+                       simp: vs_all_heap_simps)
+  apply (wpsimp wp: non_overlapping_merge_refills_non_zero_refills)
+  done
+
+lemma refill_budget_check_non_zero_refills_helper:
+  "\<lbrakk>0 < u \<and> r_time (hd refills) < MAX_RELEASE_TIME\<rbrakk> \<Longrightarrow>
+   \<lbrace>\<lambda>s. all_sp_valid_refills_but_MIN_BUDGET_in_head_no_overflow sc_ptr s
+        \<and> pred_map (\<lambda>cfg. refills_unat_sum (scrc_refills cfg) = unat (scrc_budget cfg))
+                    (sc_refill_cfgs_of s) sc_ptr
+        \<and> (pred_map (\<lambda>cfg. r_time (scrc_refill_hd cfg) < MAX_RELEASE_TIME) (sc_refill_cfgs_of s) sc_ptr
+           \<longrightarrow> pred_map (\<lambda>cfg. u < r_amount (scrc_refill_hd cfg)) (sc_refill_cfgs_of s) sc_ptr)
+        \<and> (\<exists>sc n. ko_at (SchedContext sc n) csc_ptr s \<and> refills = sc_refills sc)\<rbrace>
+   do y \<leftarrow> update_refill_hd csc_ptr (r_time_update (\<lambda>t. t + u) \<circ> r_amount_update (\<lambda>m. m - u));
+      schedule_used csc_ptr \<lparr>r_time = r_time (refill_hd sc) + sc_period sc, r_amount = u\<rparr>
+   od
+   \<lbrace>\<lambda>_ s. pred_map (\<lambda>cfg. \<forall>refill \<in> set (scrc_refills cfg). 0 < unat (r_amount refill))
+                    (sc_refill_cfgs_of s) sc_ptr\<rbrace>"
+  apply (wpsimp wp: schedule_used_non_zero_refills set_refills_wp get_refills_wp
+              simp: update_refill_hd_rewrite)
+  apply (clarsimp simp: vs_all_heap_simps obj_at_def)
+  apply (intro conjI impI allI)
+     apply (subst unat_sub)
+      apply fastforce
+     apply (clarsimp simp: word_less_nat_alt)
+    apply (simp add: list.set_sel(2))
+   apply (fastforce dest: refill_budget_check_refills_unat_sum_word_helper
+                    simp: refills_unat_sum_def)
+  apply (clarsimp simp: word_less_nat_alt)
   done
 
 lemma refill_budget_check_valid_refills[wp]:
@@ -9384,89 +9711,98 @@ lemma refill_budget_check_valid_refills[wp]:
 
   apply (rule_tac R1="\<lambda>s. pred_map (\<lambda>cfg. refills_unat_sum (scrc_refills cfg)
                                            = unat (scrc_budget cfg))
-                                   (sc_refill_cfgs_of s) csc_ptr"
+                                   (sc_refill_cfgs_of s) sc_ptr"
                in hoare_pre_add[THEN iffD2, simplified pred_conj_def])
    apply (clarsimp simp: vs_all_heap_simps)
    apply (frule valid_refills_refills_unat_sum_equals_budget
           ; (fastforce simp: )?)
    apply (clarsimp simp: sc_valid_refills_def vs_all_heap_simps)
 
-  apply (rule_tac B="\<lambda>usage' s. \<not> round_robin (cur_sc s) s
-                                \<and> all_sp_valid_refills_but_MIN_BUDGET_in_head_no_overflow (cur_sc s) s
+  apply (rule_tac B="\<lambda>usage' s. \<not> round_robin sc_ptr s
+                                \<and> all_sp_valid_refills_but_MIN_BUDGET_in_head_no_overflow sc_ptr s
                                 \<and> pred_map (\<lambda>cfg. refills_unat_sum (scrc_refills cfg)
                                                    = unat (scrc_budget cfg))
-                                           (sc_refill_cfgs_of s) (cur_sc s)
+                                           (sc_refill_cfgs_of s) sc_ptr
                                 \<and> pred_map (\<lambda>cfg. unat (r_time (hd (scrc_refills cfg)))
                                                    + 4 * unat MAX_PERIOD
                                                   \<le> unat max_time)
-                                           (sc_refill_cfgs_of s) (cur_sc s) \<and> cur_sc s = csc_ptr
+                                           (sc_refill_cfgs_of s) (cur_sc s)
+                                \<and> cur_sc s = sc_ptr
                                 \<and> (pred_map (\<lambda>cfg. r_time (hd (scrc_refills cfg)) < MAX_RELEASE_TIME)
-                                            (sc_refill_cfgs_of s) (cur_sc s)
+                                            (sc_refill_cfgs_of s) sc_ptr
                                    \<longrightarrow> pred_map (\<lambda>cfg. usage' < r_amount (hd (scrc_refills cfg)))
-                                                (sc_refill_cfgs_of s) (cur_sc s))"
+                                                (sc_refill_cfgs_of s) sc_ptr)"
                in hoare_seq_ext[rotated])
 
-    apply (intro hoare_vcg_conj_lift_pre_fix
-           ; (solves handle_overrun_loop_simple)?)
-         apply (wpsimp wp: handle_overrun_loop_refills_sum)
+   apply (intro hoare_vcg_conj_lift_pre_fix
+          ; (solves handle_overrun_loop_simple)?)
+          apply (wpsimp wp: handle_overrun_loop_refills_sum)
+          apply (fastforce simp: sc_valid_refills_def vs_all_heap_simps)
+         apply (wpsimp wp: handle_overrun_loop_ordered_disjoint)
          apply (fastforce simp: sc_valid_refills_def vs_all_heap_simps)
-        apply (wpsimp wp: handle_overrun_loop_ordered_disjoint)
+        apply (wpsimp wp: handle_overrun_loop_window)
         apply (fastforce simp: sc_valid_refills_def vs_all_heap_simps)
-       apply (wpsimp wp: handle_overrun_loop_window)
-       apply (fastforce simp: sc_valid_refills_def vs_all_heap_simps)
-      apply (wpsimp wp: handle_overrun_loop_length)
+       apply (wpsimp wp: handle_overrun_loop_length)
+       apply (clarsimp simp: sc_valid_refills_def vs_all_heap_simps)
+      apply (wpsimp wp: handle_overrun_loop_non_zero_refills)
       apply (clarsimp simp: sc_valid_refills_def vs_all_heap_simps)
      apply (wpsimp wp: handle_overrun_loop_refills_unat_sum_equals_budget)
      apply (clarsimp simp: sc_valid_refills_def vs_all_heap_simps)
     apply (wpsimp wp: handle_overrun_loop_head_bound)
     apply (fastforce simp: sc_valid_refills_def vs_all_heap_simps)
    apply (clarsimp simp: handle_overrun_loop_def)
-   apply (wpsimp wp: valid_whileLoop[where I="\<lambda>_ s. pred_map \<top> (scs_of s) (cur_sc s)"])
+   apply (wpsimp wp: valid_whileLoop[where I="\<lambda>_ s. pred_map \<top> (scs_of s) (cur_sc s)
+                                                    \<and> sc_ptr = cur_sc s"])
     apply (fastforce simp: head_time_buffer_true_imp_unat_buffer vs_all_heap_simps word_less_nat_alt
                            word_le_nat_alt)
    apply (clarsimp simp: vs_all_heap_simps)
 
-  apply (rule_tac R1="\<lambda>s. pred_map (\<lambda>cfg. no_overflow (scrc_refills cfg)) (sc_refill_cfgs_of s) (cur_sc s)"
+  apply (rule_tac R1="\<lambda>s. pred_map (\<lambda>cfg. no_overflow (scrc_refills cfg)) (sc_refill_cfgs_of s) sc_ptr"
                in hoare_pre_add[THEN iffD2, simplified pred_conj_def])
    apply (fastforce intro!: head_time_buffer_implies_no_overflow
                       simp: vs_all_heap_simps)
 
   apply (rule hoare_seq_ext[OF _ get_refills_sp])
-  apply (rule_tac B="\<lambda>_ s. \<not> round_robin (cur_sc s) s
-                           \<and> all_sp_valid_refills_but_MIN_BUDGET_in_head (cur_sc s) s
+  apply (rule_tac B="\<lambda>_ s. \<not> round_robin sc_ptr s
+                           \<and> all_sp_valid_refills_but_MIN_BUDGET_in_head sc_ptr s
                            \<and> pred_map (\<lambda>cfg. refills_unat_sum (scrc_refills cfg)
                                               = unat (scrc_budget cfg))
-                                       (sc_refill_cfgs_of s) (cur_sc s) \<and> csc_ptr = cur_sc s"
+                                       (sc_refill_cfgs_of s) sc_ptr
+                           \<and> sc_ptr = cur_sc s"
                in hoare_seq_ext[rotated])
    apply (rule hoare_when_cases, clarsimp simp: vs_all_heap_simps)
    apply (rule hoare_seq_ext[OF _ get_sched_context_sp])
    apply (intro hoare_vcg_conj_lift_pre_fix
           ; (solves schedule_used_simple)?)
 
-         apply (find_goal \<open>match conclusion in "\<lbrace>_\<rbrace> head_insufficient_loop _ \<lbrace>\<lambda>_. _\<rbrace>" \<Rightarrow> \<open>-\<close>\<close>)
-         apply (rule_tac Q="\<lambda>_ s. \<not> round_robin sc_ptr s \<and> sp_valid_refills_unbundled sc_ptr s"
-                      in hoare_strengthen_post[rotated])
-          apply (fastforce simp: valid_refills_def vs_all_heap_simps)
-         apply (intro hoare_vcg_conj_lift_pre_fix
-                ; (solves head_insufficient_loop_simple)?)
-              apply (wpsimp wp: head_insufficient_loop_refills_sum)
+          apply (find_goal \<open>match conclusion in "\<lbrace>_\<rbrace> head_insufficient_loop _ \<lbrace>\<lambda>_. _\<rbrace>" \<Rightarrow> \<open>-\<close>\<close>)
+          apply (rule_tac Q="\<lambda>_ s. \<not> round_robin sc_ptr s \<and> sp_valid_refills_unbundled sc_ptr s"
+                       in hoare_strengthen_post[rotated])
+           apply (fastforce simp: valid_refills_def vs_all_heap_simps)
+          apply (intro hoare_vcg_conj_lift_pre_fix
+                 ; (solves head_insufficient_loop_simple)?)
+                apply (wpsimp wp: head_insufficient_loop_refills_sum)
+                apply (clarsimp simp: vs_all_heap_simps word_le_nat_alt)
+               apply (wpsimp wp: head_insufficient_loop_ordered_disjoint)
+               apply (clarsimp simp: vs_all_heap_simps word_le_nat_alt)
+              apply (wpsimp wp: head_insufficient_loop_no_overflow)
               apply (clarsimp simp: vs_all_heap_simps word_le_nat_alt)
-             apply (wpsimp wp: head_insufficient_loop_ordered_disjoint)
+             apply (wpsimp wp: head_insufficient_loop_refills_window)
              apply (clarsimp simp: vs_all_heap_simps word_le_nat_alt)
-            apply (wpsimp wp: head_insufficient_loop_no_overflow)
+            apply (wpsimp wp: head_insufficient_loop_MIN_BUDGET_in_head)
             apply (clarsimp simp: vs_all_heap_simps word_le_nat_alt)
-           apply (wpsimp wp: head_insufficient_loop_refills_window)
+           apply (wpsimp wp: head_insufficient_loop_length_bounded)
            apply (clarsimp simp: vs_all_heap_simps word_le_nat_alt)
-          apply (wpsimp wp: head_insufficient_loop_MIN_BUDGET_in_head)
+          apply (wpsimp wp: head_insufficient_loop_non_zero_refills)
           apply (clarsimp simp: vs_all_heap_simps word_le_nat_alt)
-         apply (wpsimp wp: head_insufficient_loop_length_bounded)
-         apply (clarsimp simp: vs_all_heap_simps word_le_nat_alt)
-        apply (wpsimp wp: refill_budget_check_refills_sum_helper)
-       apply (wpsimp wp: refill_budget_check_ordered_disjoint_helper', fastforce+)
-      apply (wpsimp wp: refill_budget_check_no_overflow', fastforce+)
-     apply (wpsimp wp: refill_budget_check_window_helper, fastforce+)
-    apply (wpsimp wp: refill_budget_check_length_helper)
+         apply (wpsimp wp: refill_budget_check_refills_sum_helper)
+        apply (wpsimp wp: refill_budget_check_ordered_disjoint_helper', fastforce+)
+       apply (wpsimp wp: refill_budget_check_no_overflow', fastforce+)
+      apply (wpsimp wp: refill_budget_check_window_helper, fastforce+)
+     apply (wpsimp wp: refill_budget_check_length_helper)
+    apply (wpsimp wp: refill_budget_check_non_zero_refills_helper)
    apply (wpsimp wp: refill_budget_check_refills_unat_sum_helper, fastforce+)
+  apply (clarsimp simp: obj_at_def)
   apply (wpsimp wp: set_refills_wp get_refills_wp
               simp: vs_all_heap_simps update_sched_context_set_refills_rewrite update_refill_hd_rewrite)
   done
@@ -9638,6 +9974,85 @@ lemma refill_unblock_check_no_overflow_helper2:
   apply (case_tac "sc_refills sc"; clarsimp)
   done
 
+lemma merge_refills_refills_unat_sum_equals_unat_budget:
+  "\<lbrace>\<lambda>s. pred_map (\<lambda>cfg. refills_unat_sum (scrc_refills cfg) = unat (scrc_budget cfg))
+                      (sc_refill_cfgs_of s) sc_ptr
+        \<and> (sc_ptr' = sc_ptr \<longrightarrow> pred_map (\<lambda>cfg. 1 < length (scrc_refills cfg))
+                                         (sc_refill_cfgs_of s) sc_ptr)\<rbrace>
+   merge_refills sc_ptr'
+   \<lbrace>\<lambda>_ s. pred_map (\<lambda>cfg. refills_unat_sum (scrc_refills cfg) = unat (scrc_budget cfg))
+                   (sc_refill_cfgs_of s) sc_ptr\<rbrace>"
+  apply merge_refills_simple
+  apply (clarsimp simp: refills_unat_sum_def)
+  apply (rename_tac sc n)
+  apply (case_tac "sc_refills sc"; simp?)
+  apply (rename_tac a list)
+  apply (subst unat_add_lem'')
+   apply (prop_tac "unat (r_amount (hd list)) \<le> sum_list (map unat (map r_amount list))")
+    apply (fastforce intro: member_le_sum_list)
+   apply (rule_tac y="unat (sc_budget sc)" in order_trans)
+    apply fastforce
+   apply simp
+  apply (case_tac list; simp)
+  done
+
+lemma merge_refills_non_zero_refills:
+  "\<lbrace>\<lambda>s. pred_map (\<lambda>cfg. \<forall>refill\<in>set (scrc_refills cfg). 0 < unat (r_amount refill))
+                      (sc_refill_cfgs_of s) sc_ptr
+        \<and> (sc_ptr' = sc_ptr
+           \<longrightarrow> pred_map (\<lambda>cfg. scrc_refills cfg \<noteq> []) (sc_refill_cfgs_of s) sc_ptr
+               \<and> pred_map (\<lambda>cfg. refills_unat_sum (scrc_refills cfg) \<le> unat (scrc_budget cfg))
+                          (sc_refill_cfgs_of s) sc_ptr
+               \<and> the (refill_head_overlapping sc_ptr s))\<rbrace>
+    merge_refills sc_ptr'
+    \<lbrace>\<lambda>_ s. pred_map (\<lambda>cfg. \<forall>refill\<in>set (scrc_refills cfg). 0 < unat (r_amount refill))
+                     (sc_refill_cfgs_of s) sc_ptr\<rbrace>"
+  apply merge_refills_simple
+  apply (intro conjI impI)
+   apply (frule refill_head_overlapping_true_imp_length_at_least_two)
+    apply (clarsimp simp: vs_all_heap_simps)
+   apply (subst unat_add_lem'')
+    apply (rule_tac y="unat (sc_budget sc)" in order_trans)
+     apply (case_tac "sc_refills sc"; clarsimp)
+     apply (clarsimp simp: refills_unat_sum_cons)
+     apply (rule_tac y="unat (sc_budget sc)" in order_trans)
+      apply (prop_tac "unat (r_amount (hd list)) \<le> refills_unat_sum list")
+       apply (prop_tac "hd list \<in> set list")
+        apply (clarsimp simp: vs_all_heap_simps)
+       apply (frule_tac refill="hd list" in refills_unat_sum_member_bound[rotated])
+        apply (fastforce dest: refills_unat_sum_member_bound
+                         simp: vs_all_heap_simps)
+       apply fast
+      apply linarith
+     apply fastforce
+    apply simp
+   apply (clarsimp simp: vs_all_heap_simps)
+  apply (metis list.sel(2) list.set_sel(2))
+  done
+
+lemma refill_head_overlapping_loop_non_zero_refills:
+  "\<lbrace>\<lambda>s. pred_map (\<lambda>cfg. \<forall>refill \<in> set (scrc_refills cfg). 0 < unat (r_amount refill))
+                      (sc_refill_cfgs_of s) sc_ptr
+        \<and> (sc_ptr' = sc_ptr
+           \<longrightarrow>  pred_map (\<lambda>cfg. scrc_refills cfg \<noteq> []) (sc_refill_cfgs_of s) sc_ptr
+                \<and> pred_map (\<lambda>cfg. refills_unat_sum (scrc_refills cfg) = unat (scrc_budget cfg))
+                        (sc_refill_cfgs_of s) sc_ptr)\<rbrace>
+   refill_head_overlapping_loop sc_ptr'
+   \<lbrace>\<lambda>_ s. pred_map (\<lambda>cfg. \<forall>refill \<in> set (scrc_refills cfg). 0 < unat (r_amount refill))
+                   (sc_refill_cfgs_of s) sc_ptr\<rbrace>"
+  (is "\<lbrace>?P\<rbrace> _ \<lbrace>_\<rbrace>")
+  apply (clarsimp simp: refill_head_overlapping_loop_def)
+  apply (rule_tac I="\<lambda>_. ?P" in valid_whileLoop; fastforce?)
+  apply (intro hoare_vcg_conj_lift_pre_fix; (solves merge_refills_simple)?)
+   apply (wpsimp wp: merge_refills_non_zero_refills)
+   apply (clarsimp simp: vs_all_heap_simps)
+  apply (rule hoare_imp_helper; (solves merge_refills_simple)?)
+  apply (intro hoare_vcg_conj_lift_pre_fix; (solves merge_refills_simple)?)
+  apply (wpsimp wp: merge_refills_refills_unat_sum_equals_unat_budget)
+  apply (fastforce dest: refill_head_overlapping_true_imp_length_at_least_two
+                   simp: vs_all_heap_simps)
+  done
+
 lemma refill_unblock_check_valid_refills[wp]:
    "\<lbrace>valid_refills p and current_time_bounded 1\<rbrace>
     refill_unblock_check sc_ptr
@@ -9671,43 +10086,50 @@ lemma refill_unblock_check_valid_refills[wp]:
 
   apply (intro hoare_vcg_conj_lift_pre_fix
          ; (solves refill_head_overlapping_loop_simple)?)
-       apply (wpsimp wp: refill_head_overlapping_loop_refills_sum set_refills_wp get_refills_wp)
+        apply (wpsimp wp: refill_head_overlapping_loop_refills_sum set_refills_wp get_refills_wp)
+        apply (clarsimp simp: vs_all_heap_simps sc_valid_refills_def obj_at_def)
+        apply (rename_tac sc n)
+        apply (case_tac "sc_refills sc"; clarsimp)
+       apply (wpsimp wp: refill_head_overlapping_loop_ordered_disjoint_strong
+                         set_refills_wp get_refills_wp)
        apply (clarsimp simp: vs_all_heap_simps sc_valid_refills_def obj_at_def)
+       apply (intro conjI impI allI)
+          apply (blast dest: ordered_disjoint_sublist)
+         apply (fastforce intro: refill_unblock_check_no_overflow_helper)
+        apply (fastforce intro: refill_unblock_check_no_overflow_helper2)
+       apply (clarsimp simp: refills_unat_sum_def)
        apply (rename_tac sc n)
        apply (case_tac "sc_refills sc"; clarsimp)
-      apply (wpsimp wp: refill_head_overlapping_loop_ordered_disjoint_strong
-                        set_refills_wp get_refills_wp)
+      apply (wpsimp wp: refill_head_overlapping_loop_no_overflow set_refills_wp get_refills_wp)
       apply (clarsimp simp: vs_all_heap_simps sc_valid_refills_def obj_at_def)
-      apply (intro conjI impI allI)
-         apply (blast dest: ordered_disjoint_sublist)
-        apply (fastforce intro: refill_unblock_check_no_overflow_helper)
-       apply (fastforce intro: refill_unblock_check_no_overflow_helper2)
-      apply (clarsimp simp: refills_unat_sum_def)
-      apply (rename_tac sc n)
-      apply (case_tac "sc_refills sc"; clarsimp)
-     apply (wpsimp wp: refill_head_overlapping_loop_no_overflow set_refills_wp get_refills_wp)
+      apply (fastforce intro: refill_unblock_check_no_overflow_helper
+                              refill_unblock_check_no_overflow_helper2)
+     apply (wpsimp wp: refill_head_overlapping_loop_window set_refills_wp get_refills_wp)
      apply (clarsimp simp: vs_all_heap_simps sc_valid_refills_def obj_at_def)
-     apply (fastforce intro: refill_unblock_check_no_overflow_helper
-                             refill_unblock_check_no_overflow_helper2)
-    apply (wpsimp wp: refill_head_overlapping_loop_window set_refills_wp get_refills_wp)
-    apply (clarsimp simp: vs_all_heap_simps sc_valid_refills_def obj_at_def)
-    apply (intro conjI impI)
-     prefer 2
-     apply (fastforce intro: refill_unblock_check_no_overflow_helper
-                             refill_unblock_check_no_overflow_helper2)
-    apply (clarsimp simp: window_def refill_ready_def word_le_nat_alt current_time_bounded_def)
-    apply (prop_tac "last (tl (sc_refills sca)) = refill_tl sca")
-     using last_tl apply blast
-    apply (prop_tac "unat (cur_time s + kernelWCET_ticks)
-                     = unat (cur_time s) + unat kernelWCET_ticks")
-     apply (subst unat_add_lem', simp add: max_word_def, simp)
-    apply fastforce
-   apply (wpsimp wp: refill_head_overlapping_loop_hd_r_amount set_refills_wp get_refills_wp)
-   apply (clarsimp simp: vs_all_heap_simps sc_valid_refills_def obj_at_def refills_unat_sum_def)
-   apply (rename_tac sc n)
-   apply (case_tac "sc_refills sc"; clarsimp)
-  apply (wpsimp wp: refill_head_overlapping_loop_length set_refills_wp get_refills_wp)
+     apply (intro conjI impI)
+      prefer 2
+      apply (fastforce intro: refill_unblock_check_no_overflow_helper
+                              refill_unblock_check_no_overflow_helper2)
+     apply (clarsimp simp: window_def refill_ready_def word_le_nat_alt current_time_bounded_def)
+     apply (prop_tac "last (tl (sc_refills sca)) = refill_tl sca")
+      using last_tl apply blast
+     apply (prop_tac "unat (cur_time s + kernelWCET_ticks)
+                      = unat (cur_time s) + unat kernelWCET_ticks")
+      apply (subst unat_add_lem', simp add: max_word_def, simp)
+     apply fastforce
+    apply (wpsimp wp: refill_head_overlapping_loop_hd_r_amount set_refills_wp get_refills_wp)
+    apply (clarsimp simp: vs_all_heap_simps sc_valid_refills_def obj_at_def refills_unat_sum_def)
+    apply (rename_tac sc n)
+    apply (case_tac "sc_refills sc"; clarsimp)
+   apply (wpsimp wp: refill_head_overlapping_loop_length set_refills_wp get_refills_wp)
+   apply (clarsimp simp: vs_all_heap_simps sc_valid_refills_def obj_at_def)
+  apply (wpsimp wp: refill_head_overlapping_loop_non_zero_refills set_refills_wp get_refills_wp)
   apply (clarsimp simp: vs_all_heap_simps sc_valid_refills_def obj_at_def)
+  apply (rename_tac sc n)
+  apply (intro conjI impI)
+   apply (simp add: list.set_sel(2))
+  apply (clarsimp simp: refills_unat_sum_def)
+  apply (case_tac "sc_refills sc"; clarsimp)
   done
 
 lemma refill_unblock_check_is_refill_ready[wp]:
@@ -10357,12 +10779,14 @@ lemma refill_budget_check_is_refill_sufficient:
                in hoare_seq_ext)
    apply (subst is_refill_sufficient_0_alt)
    apply (wpsimp wp: head_insufficient_loop_MIN_BUDGET_in_head)
-    apply (fastforce simp: vs_all_heap_simps word_le_nat_alt)
-   apply (intro hoare_vcg_conj_lift_pre_fix; (solves head_insufficient_loop_simple)?)
-   apply (wpsimp wp: schedule_used_refills_unat_sum set_refills_wp get_refills_wp
-               simp: update_refill_hd_rewrite)
-   apply (fastforce dest!: refill_budget_check_refills_unat_sum_word_helper
-                     simp: refills_unat_sum_def vs_all_heap_simps obj_at_def sc_valid_refills_def)
+   apply (fastforce simp: vs_all_heap_simps word_le_nat_alt)
+  apply (intro hoare_vcg_conj_lift_pre_fix; (solves head_insufficient_loop_simple)?)
+   apply (rule_tac f=cur_sc in hoare_lift_Pf2)
+    apply (wpsimp wp: schedule_used_refills_unat_sum set_refills_wp get_refills_wp
+                simp: update_refill_hd_rewrite)
+    apply (fastforce dest!: refill_budget_check_refills_unat_sum_word_helper
+                      simp: refills_unat_sum_def vs_all_heap_simps obj_at_def sc_valid_refills_def)
+   apply wpsimp
   apply wpsimp
   done
 
@@ -10941,59 +11365,62 @@ lemma refill_budget_check_bounded_release_time:
 
   apply (rule_tac R1="\<lambda>s. pred_map (\<lambda>cfg. refills_unat_sum (scrc_refills cfg)
                                            = unat (scrc_budget cfg))
-                                   (sc_refill_cfgs_of s) csc_ptr"
+                                   (sc_refill_cfgs_of s) sc_ptr"
                in hoare_pre_add[THEN iffD2, simplified pred_conj_def])
    apply (clarsimp simp: vs_all_heap_simps)
    apply (frule valid_refills_refills_unat_sum_equals_budget
           ; (fastforce simp: )?)
    apply (clarsimp simp: sc_valid_refills_def vs_all_heap_simps)
 
-  apply (rule_tac B="\<lambda>usage' s. \<not> round_robin (cur_sc s) s
-                                \<and> all_sp_valid_refills_but_MIN_BUDGET_in_head_no_overflow (cur_sc s) s
+  apply (rule_tac B="\<lambda>usage' s. \<not> round_robin sc_ptr s
+                                \<and> all_sp_valid_refills_but_MIN_BUDGET_in_head_no_overflow sc_ptr s
                                 \<and> pred_map (\<lambda>cfg. refills_unat_sum (scrc_refills cfg)
                                                    = unat (scrc_budget cfg))
-                                            (sc_refill_cfgs_of s) (cur_sc s)
+                                            (sc_refill_cfgs_of s) sc_ptr
                                 \<and> pred_map (\<lambda>cfg. unat (r_time (hd (scrc_refills cfg)))
                                                    + 4 * unat MAX_PERIOD
                                                    \<le> unat max_time)
-                                            (sc_refill_cfgs_of s) (cur_sc s) \<and> cur_sc s = csc_ptr
+                                            (sc_refill_cfgs_of s) (cur_sc s)
+                                \<and> cur_sc s = sc_ptr
                                 \<and> (pred_map (\<lambda>cfg. r_time (hd (scrc_refills cfg)) < MAX_RELEASE_TIME)
-                                             (sc_refill_cfgs_of s) (cur_sc s)
+                                             (sc_refill_cfgs_of s) sc_ptr
                                    \<longrightarrow> pred_map (\<lambda>cfg. usage' < r_amount (hd (scrc_refills cfg)))
-                                                (sc_refill_cfgs_of s) (cur_sc s))
-"
+                                                (sc_refill_cfgs_of s) sc_ptr)"
                in hoare_seq_ext[rotated])
-    apply (intro hoare_vcg_conj_lift_pre_fix
-           ; (solves handle_overrun_loop_simple)?)
-         apply (wpsimp wp: handle_overrun_loop_refills_sum)
+   apply (intro hoare_vcg_conj_lift_pre_fix
+          ; (solves handle_overrun_loop_simple)?)
+          apply (wpsimp wp: handle_overrun_loop_refills_sum)
+          apply (fastforce simp: sc_valid_refills_def vs_all_heap_simps)
+         apply (wpsimp wp: handle_overrun_loop_ordered_disjoint)
          apply (fastforce simp: sc_valid_refills_def vs_all_heap_simps)
-        apply (wpsimp wp: handle_overrun_loop_ordered_disjoint)
+        apply (wpsimp wp: handle_overrun_loop_window)
         apply (fastforce simp: sc_valid_refills_def vs_all_heap_simps)
-       apply (wpsimp wp: handle_overrun_loop_window)
-       apply (fastforce simp: sc_valid_refills_def vs_all_heap_simps)
-     apply (wpsimp wp: handle_overrun_loop_length)
+       apply (wpsimp wp: handle_overrun_loop_length)
+       apply (clarsimp simp: sc_valid_refills_def vs_all_heap_simps)
+      apply (wpsimp wp: handle_overrun_loop_non_zero_refills)
+      apply (clarsimp simp: sc_valid_refills_def vs_all_heap_simps)
+     apply (wpsimp wp: handle_overrun_loop_refills_unat_sum_equals_budget)
      apply (clarsimp simp: sc_valid_refills_def vs_all_heap_simps)
-    apply (wpsimp wp: handle_overrun_loop_refills_unat_sum_equals_budget)
-    apply (clarsimp simp: sc_valid_refills_def vs_all_heap_simps)
-   apply (wpsimp wp: handle_overrun_loop_head_bound)
-   apply (fastforce simp: sc_valid_refills_def vs_all_heap_simps)
+    apply (wpsimp wp: handle_overrun_loop_head_bound)
+    apply (fastforce simp: sc_valid_refills_def vs_all_heap_simps)
    apply (clarsimp simp: handle_overrun_loop_def)
-   apply (wpsimp wp: valid_whileLoop[where I="\<lambda>_ s. pred_map \<top> (scs_of s) (cur_sc s)"])
+   apply (wpsimp wp: valid_whileLoop[where I="\<lambda>_ s. pred_map \<top> (scs_of s) (cur_sc s)
+                                                    \<and> sc_ptr = cur_sc s"])
     apply (fastforce simp: head_time_buffer_true_imp_unat_buffer vs_all_heap_simps word_less_nat_alt
                            word_le_nat_alt is_sc_obj_def)
    apply (clarsimp simp: vs_all_heap_simps)
 
-  apply (rule_tac R1="\<lambda>s. pred_map (\<lambda>cfg. no_overflow (scrc_refills cfg)) (sc_refill_cfgs_of s) (cur_sc s)"
+  apply (rule_tac R1="\<lambda>s. pred_map (\<lambda>cfg. no_overflow (scrc_refills cfg)) (sc_refill_cfgs_of s) sc_ptr"
                in hoare_pre_add[THEN iffD2, simplified pred_conj_def])
    apply (fastforce intro!: head_time_buffer_implies_no_overflow simp: vs_all_heap_simps)
 
   apply (rule hoare_seq_ext[OF _ get_refills_sp])
   apply (rule_tac B="\<lambda>_ s. \<not> round_robin (cur_sc s) s
-                           \<and> all_sp_valid_refills_but_MIN_BUDGET_in_head (cur_sc s) s
+                           \<and> all_sp_valid_refills_but_MIN_BUDGET_in_head sc_ptr s
                            \<and> pred_map (\<lambda>cfg. refills_unat_sum (scrc_refills cfg)
                                               = unat (scrc_budget cfg))
-                                       (sc_refill_cfgs_of s) (cur_sc s)
-                           \<and> csc_ptr = cur_sc s
+                                       (sc_refill_cfgs_of s) sc_ptr
+                           \<and> sc_ptr = cur_sc s
                            \<and> pred_map (\<lambda>cfg. unat (r_time (scrc_refill_hd cfg)) + 3 * unat MAX_PERIOD
                                              \<le> unat max_time)
                                       (sc_refill_cfgs_of s) (cur_sc s)"
@@ -11002,11 +11429,12 @@ lemma refill_budget_check_bounded_release_time:
     apply ( clarsimp simp: vs_all_heap_simps current_time_bounded_def)
    apply (rule hoare_seq_ext[OF _ get_sched_context_sp])
    apply (intro hoare_vcg_conj_lift_pre_fix; (solves schedule_used_simple)?)
-          apply (wpsimp wp: refill_budget_check_refills_sum_helper)
-         apply (wpsimp wp: refill_budget_check_ordered_disjoint_helper', fastforce+)
-        apply (wpsimp wp: refill_budget_check_no_overflow', fastforce+)
-       apply (wpsimp wp: refill_budget_check_window_helper, fastforce+)
-      apply (wpsimp wp: refill_budget_check_length_helper)
+           apply (wpsimp wp: refill_budget_check_refills_sum_helper)
+          apply (wpsimp wp: refill_budget_check_ordered_disjoint_helper', fastforce+)
+         apply (wpsimp wp: refill_budget_check_no_overflow', fastforce+)
+        apply (wpsimp wp: refill_budget_check_window_helper, fastforce+)
+       apply (wpsimp wp: refill_budget_check_length_helper)
+      apply (wpsimp wp: refill_budget_check_non_zero_refills_helper)
      apply (wpsimp wp: refill_budget_check_refills_unat_sum_helper, fastforce+)
     apply wpsimp
    apply (wpsimp wp: refill_budget_check_schedule_used_r_time_helper, fastforce+)
